cleaning up riscv dialect

LLVM-RISCV/examples/add.c
@@ -12,6 +12,8 @@ int64_t add_64(int64_t a, int64_t b) {
     return a + b;
 }
 
+
+
 int main () {
     int a = rand();
     int b = rand(); 
