RiscvDialect/Peephole_Optimizations/llvm_riscv.lean
@@ -7,28 +7,112 @@ import SSA.Projects.InstCombine.LLVM.Semantics
 open LLVM
 
 /- - this file is stil in progress and tried to modell riscv and llvm within one context.
-Didnt continue implementing this so far.-/
+implementation is very minimal in terms of instruction almost only one to one lowering r.-/
 
 namespace riscv.semantics
 
 def RTYPE_pure64_RISCV_ADD (rs2_val : BitVec 64) (rs1_val : BitVec 64) :BitVec 64 :=
       BitVec.add rs1_val rs2_val
 
+def RTYPE_pure64_RISCV_SUB (rs2_val : BitVec 64) (rs1_val : BitVec 64) : BitVec 64 :=
+    BitVec.sub rs1_val rs2_val
+
+def RTYPE_pure64_RISCV_AND (rs2_val : BitVec 64) (rs1_val : BitVec 64) : BitVec 64 :=
+      BitVec.and rs2_val rs1_val
+
+def RTYPE_pure64_RISCV_XOR(rs2_val : BitVec 64) (rs1_val : BitVec 64) : BitVec 64 :=
+      BitVec.xor rs2_val rs1_val
+
+def RTYPE_pure64_RISCV_OR(rs2_val : BitVec 64) (rs1_val : BitVec 64) : BitVec 64 :=
+      BitVec.or rs2_val rs1_val
+
+def RTYPE_pure64_RISCV_SLL (rs2_val : BitVec 64) (rs1_val : BitVec 64) : BitVec 64 :=
+       let shamt := (BitVec.extractLsb 5 0 rs2_val).toNat;
+       BitVec.shiftLeft rs1_val shamt
+
+def RTYPE_pure64_RISCV_SRL (rs2_val : BitVec 64) (rs1_val : BitVec 64) : BitVec 64 :=
+      let shamt := (BitVec.extractLsb 5 0 rs2_val).toNat;
+      BitVec.ushiftRight rs1_val shamt
+
+def RTYPE_pure64_RISCV_SRA (rs2_val : BitVec 64) (rs1_val : BitVec 64) :=
+BitVec.setWidth 64
+      (BitVec.extractLsb
+        (63 + (BitVec.extractLsb 5 0 rs2_val).toNat)
+        (BitVec.extractLsb 5 0 rs2_val).toNat
+        (BitVec.signExtend
+          (64 + (BitVec.extractLsb 5 0 rs2_val).toNat) rs1_val))
+
+def DIV_pure64_signed (rs2_val : BitVec 64) (rs1_val : BitVec 64) : BitVec 64 :=
+  BitVec.extractLsb' 0 64
+    (BitVec.ofInt 65
+      (max
+        (if 9223372036854775807 < if rs2_val.toInt = 0 then -1 else rs1_val.toInt.tdiv rs2_val.toInt then
+          -9223372036854775808
+        else if rs2_val.toInt = 0 then -1 else rs1_val.toInt.tdiv rs2_val.toInt)
+        0))
+
+def DIV_pure64_unsigned (rs2_val : BitVec 64) (rs1_val : BitVec 64) : BitVec 64 :=
+  BitVec.extractLsb' 0 64
+    (BitVec.ofNat 65
+      (if Int.ofNat rs2_val.toNat = 0 then -1 else (Int.ofNat rs1_val.toNat).tdiv (Int.ofNat rs2_val.toNat)).toNat)
 -- insert the llvm add semantics
 
+def REM_pure64_unsigned (rs2_val : BitVec 64) (rs1_val : BitVec 64) : BitVec 64  :=
+   BitVec.extractLsb' 0 64
+    (BitVec.ofInt 65
+      (Int.ofNat
+        (if Int.ofNat rs2_val.toNat = 0 then Int.ofNat rs1_val.toNat
+          else (Int.ofNat rs1_val.toNat).tmod (Int.ofNat rs2_val.toNat)).toNat))
+
+def REM_pure64_signed (rs2_val : BitVec 64) (rs1_val : BitVec 64) : BitVec 64  :=
+    BitVec.extractLsb' 0 64
+    (BitVec.ofInt 65
+      (Int.ofNat (if rs2_val.toInt = 0 then rs1_val.toInt else rs1_val.toInt.tmod rs2_val.toInt).toNat))
+
+def MUL_pure64_ftt (rs2_val : BitVec 64) (rs1_val : BitVec 64) : BitVec 64 :=
+  BitVec.extractLsb 63 0
+    (BitVec.extractLsb' 0 128 (BitVec.ofInt 129 (Int.ofNat (Int.mul rs1_val.toInt rs2_val.toInt).toNat)))
 end riscv.semantics
 
-namespace llvm.semantics
 
-end llvm.semantics
 
 namespace llvm.riscv
 section Dialect
 
+
 inductive Op
 |riscv.add
-|llvm.add (nswnuw : NoWrapFlags := {nsw := false, nuw := false} )
-deriving DecidableEq, Repr
+|llvm.add (width: Nat) (nswnuw : NoWrapFlags := {nsw := false, nuw := false} ) -- defines it as an optional value and if passed overwrites the default value, else default value.
+|riscv.sub
+|llvm.sub (width: Nat)(nswnuw : NoWrapFlags := {nsw := false, nuw := false} )
+|llvm.not (width: Nat)
+|riscv.const (val: Int)
+|llvm.const (width: Nat) (val: Int)
+|llvm.neg (width: Nat)
+|llvm.and (width: Nat)
+|riscv.and
+|llvm.or (width: Nat)  (disjoint : DisjointFlag := {disjoint := false} )
+|riscv.or
+|llvm.xor (width: Nat)
+|riscv.xor
+|llvm.shl (width: Nat)  (nswnuw : NoWrapFlags := {nsw := false, nuw := false} )
+|riscv.sll
+|llvm.lshr (width: Nat)(exact : ExactFlag := {exact := false} )
+|riscv.srl
+|riscv.sra
+|llvm.ashr (width: Nat) (exact : ExactFlag := {exact := false} )
+|llvm.sdiv (width: Nat) (exact : ExactFlag := {exact := false} )
+|riscv.div
+|llvm.udiv (width: Nat) (exact : ExactFlag := {exact := false} )
+|riscv.divu
+|llvm.urem (width: Nat)
+|riscv.remu
+|llvm.srem (width: Nat)
+|riscv.rem
+|llvm.mul (width: Nat)  (nswnuw : NoWrapFlags := {nsw := false, nuw := false} )
+|riscv.mul
+deriving DecidableEq, Inhabited, Lean.ToExpr
+
 
 
 inductive Ty -- here belongs what my operations operate on
@@ -47,17 +131,73 @@ abbrev llvm.riscv : Dialect where
   Op := Op -- define the avaiable operations
   Ty := Ty -- define the avaiable types
 
-@[simp, reducible]
+@[simp, reducible] -- this basically will be the contexts
 def Op.sig : Op → List Ty
 |riscv.add => [Ty.bv64, Ty.bv64]
-|llvm.add _ => [Ty.opt64, Ty.opt64]
---|llvm.add =>
+|llvm.add _ _ => [Ty.opt64, Ty.opt64] -- defines it as an optional value and if passed overwrites the default value, else default value.
+|riscv.sub => [Ty.bv64, Ty.bv64]
+|llvm.sub _ _ => [Ty.opt64, Ty.opt64]
+|llvm.not _ => [Ty.opt64]
+|riscv.const val => []
+|llvm.const _ val => []
+|llvm.neg _ => [Ty.opt64]
+|llvm.and _ => [Ty.opt64, Ty.opt64]
+|riscv.and => [Ty.bv64, Ty.bv64]
+|llvm.or _ _ => [Ty.opt64, Ty.opt64]
+|riscv.or => [Ty.bv64, Ty.bv64]
+|llvm.xor _ => [Ty.opt64, Ty.opt64]
+|riscv.xor => [Ty.bv64, Ty.bv64]
+|llvm.shl _ _ => [Ty.opt64, Ty.opt64]
+|riscv.sll => [Ty.bv64, Ty.bv64]
+|llvm.lshr _ _  => [Ty.opt64, Ty.opt64]
+|riscv.sra => [Ty.bv64, Ty.bv64]
+|riscv.srl => [Ty.bv64, Ty.bv64]
+|llvm.ashr _ _ => [Ty.opt64, Ty.opt64]
+|llvm.sdiv _ _ => [Ty.opt64, Ty.opt64]
+|riscv.div => [Ty.bv64, Ty.bv64]
+|llvm.udiv _ _ => [Ty.opt64, Ty.opt64]
+|riscv.divu => [Ty.bv64, Ty.bv64]
+|llvm.urem _  =>  [Ty.opt64, Ty.opt64]
+|riscv.remu => [Ty.bv64, Ty.bv64]
+|llvm.srem _ => [Ty.opt64, Ty.opt64]
+|riscv.rem => [Ty.bv64, Ty.bv64]
+|llvm.mul _ _ => [Ty.opt64, Ty.opt64]
+|riscv.mul => [Ty.bv64, Ty.bv64 ]
 
 
 @[simp, reducible] -- reduceable means this expression can always be expanded by the type checker when type checking
+-- output signature , part of an op
 def Op.outTy : Op  → Ty
-|riscv.add => Ty.bv64
-|llvm.add _ => Ty.opt64
+|riscv.add => .bv64
+|llvm.add _ flags => .opt64
+|riscv.sub => .bv64
+|llvm.sub _ _ => .opt64
+|llvm.not _ => .opt64
+|riscv.const val  => .bv64
+|llvm.const _ val  => .opt64
+|llvm.neg _ => .opt64
+|llvm.and _ => .opt64
+|riscv.and => .bv64
+|llvm.or _ _ => .opt64
+|riscv.or => .bv64
+|llvm.xor _ => .opt64
+|riscv.xor => .bv64
+|llvm.shl _ _ => .opt64
+|riscv.sll => .bv64
+|llvm.lshr _ _ => .opt64
+|riscv.srl => .bv64
+|riscv.sra => .bv64
+|llvm.ashr _ _ => .opt64
+|llvm.sdiv _ _ => .opt64
+|riscv.div => .bv64
+|llvm.udiv _ _ => .opt64
+|riscv.divu => .bv64
+|llvm.urem _ => .opt64
+|riscv.remu => .bv64
+|llvm.srem _ => .opt64
+|riscv.rem => .bv64
+|llvm.mul _ _ => .opt64
+|riscv.mul => .bv64
 
 @[simp, reducible]
 def Op.signature : Op → Signature (Ty) :=
@@ -65,12 +205,75 @@ def Op.signature : Op → Signature (Ty) :=
 
 instance : DialectSignature llvm.riscv := ⟨Op.signature⟩
 
-@[simp, reducible]
+
+open LLVM
+
+@[simp, reducible] -- structure is parameter to the op, then arguemtns then return type
 instance : DialectDenote (llvm.riscv) where denote
   |.riscv.add, regs, _ => riscv.semantics.RTYPE_pure64_RISCV_ADD (regs.getN 0 (by simp [DialectSignature.sig, signature]))  (regs.getN 1 (by simp [DialectSignature.sig, signature]))
-  |.llvm.add flags, regs, _  =>  LLVM.add (regs.getN 0 (by simp [DialectSignature.sig, signature])) (regs.getN 1 (by simp [DialectSignature.sig, signature])) flags
+  |.riscv.sub, regs,_  => riscv.semantics.RTYPE_pure64_RISCV_SUB (regs.getN 0 (by simp [DialectSignature.sig, signature]))  (regs.getN 1 (by simp [DialectSignature.sig, signature]))
+  |.riscv.const val, _, _ => BitVec.ofInt 64 val
+  |.riscv.and, regs, _  => riscv.semantics.RTYPE_pure64_RISCV_AND (regs.getN 0 (by simp [DialectSignature.sig, signature])) (regs.getN 1 (by simp [DialectSignature.sig, signature]))
+  |.riscv.xor, regs, _  => riscv.semantics.RTYPE_pure64_RISCV_XOR (regs.getN 0 (by simp [DialectSignature.sig, signature]))  (regs.getN 1 (by simp [DialectSignature.sig, signature]))
+  |.riscv.sll, regs, _  => riscv.semantics.RTYPE_pure64_RISCV_SLL (regs.getN 1 (by simp [DialectSignature.sig, signature]))  (regs.getN 0 (by simp [DialectSignature.sig, signature]))
+  |.riscv.or, regs, _  => riscv.semantics.RTYPE_pure64_RISCV_OR (regs.getN 0 (by simp [DialectSignature.sig, signature])) (regs.getN 1 (by simp [DialectSignature.sig, signature]))
+  |.riscv.srl, regs, _  => riscv.semantics.RTYPE_pure64_RISCV_SRL (regs.getN 1 (by simp [DialectSignature.sig, signature]))  (regs.getN 0 (by simp [DialectSignature.sig, signature]))
+  |.riscv.sra, regs, _  =>  riscv.semantics.RTYPE_pure64_RISCV_SRA (regs.getN 1 (by simp [DialectSignature.sig, signature]))  (regs.getN 0 (by simp [DialectSignature.sig, signature]))
+  |.riscv.div, regs, _  => riscv.semantics.DIV_pure64_signed (regs.getN 1 (by simp [DialectSignature.sig, signature]))  (regs.getN 0 (by simp [DialectSignature.sig, signature]))
+  |.riscv.divu, regs, _ => riscv.semantics.DIV_pure64_unsigned (regs.getN 0 (by simp [DialectSignature.sig, signature]))  (regs.getN 1 (by simp [DialectSignature.sig, signature]))
+  |.riscv.remu, regs,_  =>  riscv.semantics.REM_pure64_unsigned (regs.getN 1 (by simp [DialectSignature.sig, signature]))  (regs.getN 0 (by simp [DialectSignature.sig, signature]))
+  |.riscv.rem, regs,_ => riscv.semantics.REM_pure64_signed (regs.getN 1 (by simp [DialectSignature.sig, signature]))  (regs.getN 0 (by simp [DialectSignature.sig, signature]))
+  |.riscv.mul, regs, _ => riscv.semantics.MUL_pure64_ftt (regs.getN 0 (by simp [DialectSignature.sig, signature]))  (regs.getN 1 (by simp [DialectSignature.sig, signature]))
+  |.llvm.add _ flags, op, _  => LLVM.add (op.getN 0 (by simp [DialectSignature.sig, signature])) (op.getN 1 (by simp [DialectSignature.sig, signature])) flags
+  |.llvm.sub _ flags,op,_ => LLVM.sub (op.getN 0 (by simp [DialectSignature.sig, signature])) (op.getN 1 (by simp [DialectSignature.sig, signature])) flags
+  |.llvm.not _, op,_ => LLVM.not  (op.getN 0 (by simp [DialectSignature.sig, signature]))
+  |.llvm.neg _, op,_ => LLVM.neg (op.getN 0 (by simp [DialectSignature.sig, signature]))
+  |.llvm.and _, op,_ => LLVM.and  (op.getN 0 (by simp [DialectSignature.sig, signature])) (op.getN 1 (by simp [DialectSignature.sig, signature]))
+  |.llvm.or _ flag, op,_  => LLVM.or       (op.getN 0 (by simp [DialectSignature.sig, signature])) (op.getN 1 (by simp [DialectSignature.sig, signature])) flag
+  |.llvm.xor _, op, _  => LLVM.xor (op.getN 0 (by simp [DialectSignature.sig, signature])) (op.getN 1 (by simp [DialectSignature.sig, signature]))
+  |.llvm.shl _ flags, op,_  => LLVM.shl      (op.getN 0 (by simp [DialectSignature.sig, signature])) (op.getN 1 (by simp [DialectSignature.sig, signature])) flags
+  |.llvm.lshr _ flags, op,_  => LLVM.lshr     (op.getN 0 (by simp [DialectSignature.sig, signature])) (op.getN 1 (by simp [DialectSignature.sig, signature])) flags
+  |.llvm.ashr _ flag, op,_ => LLVM.ashr     (op.getN 0 (by simp [DialectSignature.sig, signature])) (op.getN 1 (by simp [DialectSignature.sig, signature])) flag
+  |.llvm.sdiv _ flag, op,_  => LLVM.sdiv     (op.getN 0 (by simp [DialectSignature.sig, signature])) (op.getN 1 (by simp [DialectSignature.sig, signature])) flag
+  |.llvm.udiv _ flag, op,_ => LLVM.udiv    (op.getN 0 (by simp [DialectSignature.sig, signature])) (op.getN 1 (by simp [DialectSignature.sig, signature])) flag
+  |.llvm.urem _, op, _ => LLVM.urem     (op.getN 0 (by simp [DialectSignature.sig, signature])) (op.getN 1 (by simp [DialectSignature.sig, signature]))
+  |.llvm.srem _, op,_  => LLVM.srem     (op.getN 0 (by simp [DialectSignature.sig, signature])) (op.getN 1 (by simp [DialectSignature.sig, signature]))
+  |.llvm.mul _  flags, op,_ => LLVM.mul      (op.getN 0 (by simp [DialectSignature.sig, signature])) (op.getN 1 (by simp [DialectSignature.sig, signature])) flags
+  |.llvm.const _ val, _ , _ => some (BitVec.ofInt 64 val)
+
+
+
+/-
+  |.llvm.sub _, _ => .opt64
+  |.llvm.not _ => .opt64
+  |.riscv.const val => BitVec.ofInt 64 val
+  |.llvm.neg _ => .opt64
+  |.llvm.and _ => .opt64
+  |.riscv.and => RV64.RTYPE_pure64_RISCV_AND (regs.getN 0 (by simp [DialectSignature.sig, signature])) (regs.getN 1 (by simp [DialectSignature.sig, signature]))
+  |.llvm.or _, _ => .opt64
+  |.riscv.or  => RV64.RTYPE_pure64_RISCV_OR (regs.getN 0 (by simp [DialectSignature.sig, signature])) (regs.getN 1 (by simp [DialectSignature.sig, signature]))
+  |.llvm.xor _ => .opt64
+  |.riscv.xor => .bv64
+  |.llvm.shl _, _ => .opt64
+  |.riscv.sll => .bv64
+  |.llvm.lshr _, _ => .opt64
+  |.riscv.srl => .bv64
+  |.riscv.ashr => .bv64
+  |.llvm.ashr _ _ => .opt64
+  |.llvm.sdiv _ _ => .opt64
+  |.riscv.div => .bv64
+  |.llvm.udiv _ _ => .opt64
+  |.riscv.divu => .bv64
+  |.llvm.urem _ => .opt64
+  |.riscv.remu => .bv64
+  |.llvm.srem _ => .opt64
+  |.riscv.rem => .bv64
+  |.llvm.mul _, _ => .opt64
+  |.riscv.mul => .bv64
+-/
 end Dialect
 
+-- helper functions to easier create expressions and check the parsing of a program writtin in IR style into Com and Expr.
 def riscv.add {Γ : Ctxt _} (e₁ e₂: Ctxt.Var Γ .bv64) : Expr llvm.riscv Γ .pure .bv64  :=
   Expr.mk
     (op := llvm.riscv.Op.riscv.add)
@@ -81,12 +284,118 @@ def riscv.add {Γ : Ctxt _} (e₁ e₂: Ctxt.Var Γ .bv64) : Expr llvm.riscv Γ 
 
 def llvm.add {Γ : Ctxt _} (e₁ e₂: Ctxt.Var Γ .opt64) : Expr llvm.riscv Γ .pure .opt64  :=
   Expr.mk
-    (op := llvm.riscv.Op.llvm.add)
+    (op := llvm.riscv.Op.llvm.add 64)
     (eff_le := by constructor)
     (ty_eq := rfl)
     (args := .cons e₁ <| .cons e₂ .nil)
     (regArgs := HVector.nil)
 
+def riscv.sub {Γ : Ctxt _} (e₁ e₂: Ctxt.Var Γ .bv64) : Expr llvm.riscv Γ .pure .bv64  :=
+  Expr.mk
+    (op := llvm.riscv.Op.riscv.sub)
+    (eff_le := by constructor)
+    (ty_eq := rfl)
+    (args := .cons e₁ <| .cons e₂ .nil)
+    (regArgs := HVector.nil)
+
+def llvm.sub {Γ : Ctxt _} (e₁ e₂: Ctxt.Var Γ .opt64) : Expr llvm.riscv Γ .pure .opt64  :=
+  Expr.mk
+    (op := llvm.riscv.Op.llvm.sub 64)
+    (eff_le := by constructor)
+    (ty_eq := rfl)
+    (args := .cons e₁ <| .cons e₂ .nil)
+    (regArgs := HVector.nil)
+
+def llvm.not {Γ : Ctxt _} (e₁: Ctxt.Var Γ .opt64) : Expr llvm.riscv Γ .pure .opt64  :=
+    Expr.mk
+    (op := llvm.riscv.Op.llvm.not 64)
+    (eff_le := by constructor)
+    (ty_eq := rfl)
+    (args := .cons e₁ <| .nil)
+    (regArgs := HVector.nil)
+
+def llvm.neg {Γ : Ctxt _} (e₁: Ctxt.Var Γ .opt64) : Expr llvm.riscv Γ .pure .opt64  :=
+    Expr.mk
+    (op := llvm.riscv.Op.llvm.neg 64)
+    (eff_le := by constructor)
+    (ty_eq := rfl)
+    (args := .cons e₁ <| .nil)
+    (regArgs := HVector.nil)
+
+def llvm.and {Γ : Ctxt _} (e₁ e₂: Ctxt.Var Γ .opt64) : Expr llvm.riscv Γ .pure .opt64  :=
+  Expr.mk
+    (op := llvm.riscv.Op.llvm.and 64)
+    (eff_le := by constructor)
+    (ty_eq := rfl)
+    (args := .cons e₁ <| .cons e₂ .nil)
+    (regArgs := HVector.nil)
+
+def llvm.or {Γ : Ctxt _} (e₁ e₂: Ctxt.Var Γ .opt64) : Expr llvm.riscv Γ .pure .opt64  :=
+  Expr.mk
+    (op := llvm.riscv.Op.llvm.or 64)
+    (eff_le := by constructor)
+    (ty_eq := rfl)
+    (args := .cons e₁ <| .cons e₂ .nil)
+    (regArgs := HVector.nil)
+
+def llvm.xor {Γ : Ctxt _} (e₁ e₂: Ctxt.Var Γ .opt64) : Expr llvm.riscv Γ .pure .opt64  :=
+  Expr.mk
+    (op := llvm.riscv.Op.llvm.xor 64)
+    (eff_le := by constructor)
+    (ty_eq := rfl)
+    (args := .cons e₁ <| .cons e₂ .nil)
+    (regArgs := HVector.nil)
+
+def riscv.mul {Γ : Ctxt _} (e₁ e₂: Ctxt.Var Γ .bv64) : Expr llvm.riscv Γ .pure .bv64  :=
+  Expr.mk
+    (op := llvm.riscv.Op.riscv.mul)
+    (eff_le := by constructor)
+    (ty_eq := rfl)
+    (args := .cons e₁ <| .cons e₂ .nil)
+    (regArgs := HVector.nil)
+
+def llvm.mul {Γ : Ctxt _} (e₁ e₂: Ctxt.Var Γ .opt64) : Expr llvm.riscv Γ .pure .opt64  :=
+  Expr.mk
+    (op := llvm.riscv.Op.llvm.mul 64)
+    (eff_le := by constructor)
+    (ty_eq := rfl)
+    (args := .cons e₁ <| .cons e₂ .nil)
+    (regArgs := HVector.nil)
+
+def riscv.const {Γ : Ctxt _} (n : ℤ) : Expr llvm.riscv Γ .pure .bv64  :=
+  Expr.mk
+    (op := llvm.riscv.Op.riscv.const n)
+    (eff_le := by constructor)
+    (ty_eq := rfl)
+    (args := .nil)
+    (regArgs := HVector.nil)
+
+def llvm.const {Γ : Ctxt _} (n : ℤ) : Expr llvm.riscv Γ .pure .opt64  :=
+  Expr.mk
+    (op := llvm.riscv.Op.llvm.const 64 n)
+    (eff_le := by constructor)
+    (ty_eq := rfl)
+    (args := .nil)
+    (regArgs := HVector.nil)
+
+/-
+def riscv.const {Γ : Ctxt _} (n : ℤ) : Expr llvm.riscv Γ .pure .bv64  :=
+  Expr.mk
+    (op := llvm.riscv.Op.riscv.const n)
+    (eff_le := by constructor)
+    (ty_eq := rfl)
+    (args := .nil)
+    (regArgs := HVector.nil)
+
+def llvm.const {Γ : Ctxt _} (n : ℤ) : Expr llvm.riscv Γ .pure .opt64  :=
+  Expr.mk
+    (op := llvm.riscv.Op.llvm.const 64 n)
+    (eff_le := by constructor)
+    (ty_eq := rfl)
+    (args := .nil)
+    (regArgs := HVector.nil)
+
+-/
 def mkTy : MLIR.AST.MLIRType φ → MLIR.AST.ExceptM llvm.riscv llvm.riscv.Ty
   | MLIR.AST.MLIRType.undefined s => do
     match s with
@@ -102,6 +411,34 @@ instance instTransformTy : MLIR.AST.TransformTy llvm.riscv 0 where
 def mkExpr (Γ : Ctxt _) (opStx : MLIR.AST.Op 0) :
   MLIR.AST.ReaderM (llvm.riscv) (Σ eff ty, Expr (llvm.riscv) Γ eff ty) := do
     match opStx.args with
+    | v₁Stx :: [] =>
+       let ⟨ty₁, v₁⟩ ← MLIR.AST.TypedSSAVal.mkVal Γ v₁Stx
+       match ty₁, opStx.name with
+       | .opt64 , "llvm.neg"=> -- unsure if handeld flags correctly
+              return ⟨ .pure, .opt64 ,⟨ .llvm.neg 64 , by rfl, by constructor,
+               .cons v₁ <| .nil,
+                .nil⟩⟩
+       | .opt64 , "llvm.not"=> -- unsure if handeld flags correctly
+              return ⟨ .pure, .opt64 ,⟨ .llvm.not 64 , by rfl, by constructor,
+               .cons v₁ <| .nil,
+                .nil⟩⟩
+        | .opt64 , "llvm.const"=> -- unsure if handeld flags correctly
+            let some att := opStx.attrs.getAttr "val"
+              | throw <| .unsupportedOp s!"no attirbute in constant value provided {repr opStx}"
+              match att with
+              | .int val ty => -- ides modell it as a list of 3 bools
+                --let opTy@(.opt64) ← mkTy ty -- ty.mkTy -- potential debug
+                return ⟨.pure, .opt64, ⟨
+                  .llvm.const 64 val,
+                  by
+                  simp[DialectSignature.outTy, signature]
+                ,
+                  by constructor,
+                  .nil,
+                  .nil
+                ⟩⟩
+              | _ => throw <| .unsupportedOp s!"unsupported operation {repr opStx}"
+       | _ ,_=> throw <| .unsupportedOp s!"is a one argument op but shouldnt be one, cant find a matching case  {repr opStx}"
     | v₁Stx::v₂Stx:: [] =>
         let ⟨ty₁, v₁⟩ ← MLIR.AST.TypedSSAVal.mkVal Γ v₁Stx
         let ⟨ty₂, v₂⟩ ← MLIR.AST.TypedSSAVal.mkVal Γ v₂Stx
@@ -110,8 +447,100 @@ def mkExpr (Γ : Ctxt _) (opStx : MLIR.AST.Op 0) :
               return ⟨ .pure, .bv64 ,⟨ .riscv.add, by rfl, by constructor,
                .cons v₁ <| .cons v₂ <| .nil,
                 .nil⟩⟩
+        | .bv64 , .bv64 , "sub" =>
+              return ⟨ .pure, .bv64 ,⟨ .riscv.sub, by rfl, by constructor,
+               .cons v₁ <| .cons v₂ <| .nil,
+                .nil⟩⟩
+        | .bv64 , .bv64 , "and" =>
+              return ⟨ .pure, .bv64 ,⟨ .riscv.and, by rfl, by constructor,
+               .cons v₁ <| .cons v₂ <| .nil,
+                .nil⟩⟩
+        | .bv64 , .bv64 , "xor" =>
+              return ⟨ .pure, .bv64 ,⟨ .riscv.xor, by rfl, by constructor,
+               .cons v₁ <| .cons v₂ <| .nil,
+                .nil⟩⟩
+        | .bv64 , .bv64 , "sll" =>
+              return ⟨ .pure, .bv64 ,⟨ .riscv.sll, by rfl, by constructor,
+               .cons v₁ <| .cons v₂ <| .nil,
+                .nil⟩⟩
+        | .bv64 , .bv64 , "or" =>
+              return ⟨ .pure, .bv64 ,⟨ .riscv.or, by rfl, by constructor,
+               .cons v₁ <| .cons v₂ <| .nil,
+                .nil⟩⟩
+        | .bv64 , .bv64 , "srl" =>
+              return ⟨ .pure, .bv64 ,⟨ .riscv.srl, by rfl, by constructor,
+               .cons v₁ <| .cons v₂ <| .nil,
+                .nil⟩⟩
+        | .bv64 , .bv64 , "sra" =>
+              return ⟨ .pure, .bv64 ,⟨ .riscv.sra, by rfl, by constructor,
+               .cons v₁ <| .cons v₂ <| .nil,
+                .nil⟩⟩
+        | .bv64 , .bv64 , "div" =>
+              return ⟨ .pure, .bv64 ,⟨ .riscv.div, by rfl, by constructor,
+               .cons v₁ <| .cons v₂ <| .nil,
+                .nil⟩⟩
+        | .bv64 , .bv64 , "divu" =>
+              return ⟨ .pure, .bv64 ,⟨ .riscv.divu, by rfl, by constructor,
+               .cons v₁ <| .cons v₂ <| .nil,
+                .nil⟩⟩
+        | .bv64 , .bv64 , "remu" =>
+              return ⟨ .pure, .bv64 ,⟨ .riscv.remu, by rfl, by constructor,
+               .cons v₁ <| .cons v₂ <| .nil,
+                .nil⟩⟩
+        | .bv64 , .bv64 , "rem" =>
+              return ⟨ .pure, .bv64 ,⟨ .riscv.remu, by rfl, by constructor,
+               .cons v₁ <| .cons v₂ <| .nil,
+                .nil⟩⟩
+        | .bv64 , .bv64 , "mul" =>
+              return ⟨ .pure, .bv64 ,⟨ .riscv.mul, by rfl, by constructor,
+               .cons v₁ <| .cons v₂ <| .nil,
+                .nil⟩⟩
         | .opt64 , .opt64 , "llvm.add" => -- unsure if handeld flags correctly
-              return ⟨ .pure, .opt64 ,⟨ .llvm.add , by rfl, by constructor,
+              return ⟨ .pure, .opt64 ,⟨ .llvm.add 64 , by rfl, by constructor,
+               .cons v₁ <| .cons v₂ <| .nil,
+                .nil⟩⟩
+        | .opt64 , .opt64 , "llvm.sub" => -- unsure if handeld flags correctly
+              return ⟨ .pure, .opt64 ,⟨ .llvm.sub 64 , by rfl, by constructor,
+               .cons v₁ <| .cons v₂ <| .nil,
+                .nil⟩⟩
+        | .opt64 , .opt64 , "llvm.and" => -- unsure if handeld flags correctly
+              return ⟨ .pure, .opt64 ,⟨ .llvm.and 64 , by rfl, by constructor,
+               .cons v₁ <| .cons v₂ <| .nil,
+                .nil⟩⟩
+          -- TO DO handle the attributes
+        | .opt64 , .opt64 , "llvm.or" => -- unsure if handeld flags correctly
+            let some att := opStx.attrs.getAttr "disjoint"
+              | throw <| .unsupportedOp s!"no attirbute in constant value provided {repr opStx}"
+              match att with
+              | .list  nswnuw ty => -- ides modell it as a list of 3 bools
+                --let opTy@(.opt64) ← mkTy ty -- ty.mkTy -- potential debug
+                return ⟨.pure, .opt64, ⟨
+                  .llvm.or 64 flags,
+                  by
+                  simp[DialectSignature.outTy, signature]
+                ,
+                  by constructor,
+                  .cons v₁ <| .cons v₂ <| .nil,
+                  .nil
+                ⟩⟩
+              | .int val ty => -- ides modell it as a list of 3 bools
+              return ⟨ .pure, .opt64 ,⟨ .llvm.and 64 , by rfl, by constructor,
+               .cons v₁ <| .cons v₂ <| .nil,
+                .nil⟩⟩
+        | .opt64 , .opt64 , "llvm.xor" => -- unsure if handeld flags correctly
+              return ⟨ .pure, .opt64 ,⟨ .llvm.and 64 , by rfl, by constructor,
+               .cons v₁ <| .cons v₂ <| .nil,
+                .nil⟩⟩
+        | .opt64 , .opt64 , "llvm.shl" => -- unsure if handeld flags correctly
+              return ⟨ .pure, .opt64 ,⟨ .llvm.shl 64 , by rfl, by constructor,
+               .cons v₁ <| .cons v₂ <| .nil,
+                .nil⟩⟩
+        | .opt64 , .opt64 , "llvm.srem" => -- unsure if handeld flags correctly
+              return ⟨ .pure, .opt64 ,⟨ .llvm.srem 64 , by rfl, by constructor,
+               .cons v₁ <| .cons v₂ <| .nil,
+                .nil⟩⟩
+        | .opt64 , .opt64 , "llvm.urem" => -- unsure if handeld flags correctly
+              return ⟨ .pure, .opt64 ,⟨ .llvm.urem 64 , by rfl, by constructor,
                .cons v₁ <| .cons v₂ <| .nil,
                 .nil⟩⟩
         | _ ,_, _ => throw <| .unsupportedOp s!"wrong number of arguemnts, more than 2 arguemnts  {repr opStx}"
@@ -139,7 +568,7 @@ elab "[_| " reg:mlir_region "]" : term => do
 
 end llvm.riscv
 
-open llvm.semantics
+open LLVM
 open llvm.riscv
 
 /- instead of lowering implemented by myself implement a lowering using the peephole rewriter and extend the rewriter to
@@ -164,32 +593,7 @@ def exampleRiscv : Com llvm.riscv [.bv64] .pure .bv64 :=
  def LLVMCtxtToRV (Γ : Ctxt llvm.riscv.Ty) : Ctxt llvm.riscv.Ty :=
   List.replicate Γ.length (.bv64)
 
-
 /--TO DO: ask for a shorter proof.-/
-
-/-
-    simp [LLVMCtxtToRV]
-    have hcontra2 : Γ.get? i = some (InstCombine.Ty.bitvec 64) := by exact h
-    have hcontra3: List.length Γ ≤ i → Γ.get? i  = none := by simp [List.get?]
-    have hcontra : i <  Γ.length :=  by
-      by_contra h
-      simp at h
-      have h_none : Γ.get? i = none := hcontra3 h
-      rw [hcontra2] at h_none
-      contradiction
-    have leng_eq_leng : i < List.length Γ → i < List.length (List.replicate (List.length Γ) Ty.bv) := by simp
-    have h3 : i < (List.replicate (List.length Γ) Ty.bv).length := by exact leng_eq_leng hcontra
-    have h4 : (List.replicate (List.length Γ) Ty.bv)[i] = Ty.bv → (List.replicate (List.length Γ) Ty.bv)[i]? = some Ty.bv := by
-        simp [List.get?_eq_some]
-        exact hcontra
-    apply h4
-    rfl
-
-
-
-
-
--/
 
 def LLVMVarToRV : Γ.Var (.opt64) → (LLVMCtxtToRV Γ).Var .bv64
   | ⟨i, h⟩ =>  ⟨i, by
@@ -215,7 +619,7 @@ def LLVMVarToRV : Γ.Var (.opt64) → (LLVMCtxtToRV Γ).Var .bv64
 def lowerSimpleIRInstructionDialect (e : Expr llvm.riscv Γ .pure .opt64) :  Expr llvm.riscv (LLVMCtxtToRV Γ) .pure .bv64 :=
   match e with
   | Expr.mk
-    (.llvm.add flags)
+    (.llvm.add 64 flags)
     (_)
     (_)
     (.cons e₁ <| .cons e₂ <| .nil ) -- are of type .opt64 which are option bitvector -> can either extract them and add them to the context but then need to know
@@ -225,7 +629,15 @@ def lowerSimpleIRInstructionDialect (e : Expr llvm.riscv Γ .pure .opt64) :  Exp
     (ty_eq := rfl)
     (args := .cons  (LLVMVarToRV e₁) <| .cons  (LLVMVarToRV e₂) <| .nil  )
     (regArgs := .nil)
-  --|e  =>   -- still wrong type
+  |e  =>
+    Expr.mk
+    (op := .riscv.const 0) -- for the moment hard coded to zero.
+    (eff_le := by constructor)
+    (ty_eq := rfl)
+    (args :=  .nil  )
+    (regArgs := .nil)
+
+    -- still wrong type
 
 
 def loweringLLVMtoRISCV : {Γ : Ctxt llvm.riscv.Ty} → (com : Com llvm.riscv Γ .pure (.opt64)) → Option (Com llvm.riscv (LLVMCtxtToRV Γ)  .pure (.bv64))
@@ -251,14 +663,43 @@ def exampleRiscv1 : Com llvm.riscv (Ctxt.ofList [.bv64]) .pure .bv64 :=
   "return" (%1) : ( !r64) -> ()
 }]
 
-
+ DOESNT WORK YET BECAUSE THE REWRITER DOESNT WORK FOR REFINEMENT YET
 -- problem of the peephole rewriter that he doesnt support refinements
-def loweringViaRewriter :  PeepholeRewrite llvm.riscv ([Ty.opt64]) .bv64 :=
- { lhs := [_| {
+
+def loweringViaRewriterWorks :  PeepholeRewrite llvm.riscv ([Ty.opt64]) .opt64 :=
+ {lhs := [_| {
   ^entry (%0: !i64 ):
   %1 = "llvm.add" (%0, %0) : (!i64, !i64 ) -> (!i64)
   "return" (%1) : ( !i64) -> ()
-}], rhs:=
+}], rhs := [_| {
+  ^entry (%0: !i64 ):
+  %1 = "llvm.add" (%0, %0) : (!i64, !i64 ) -> (!i64)
+  "return" (%1) : ( !i64) -> ()
+}],
+correct
+
+ }
+
+
+def loweringViaRewriterDoesntWork :  PeepholeRewrite llvm.riscv ([Ty.opt64]) .bv64 :=
+ {lhs := [_| {
+  ^entry (%0: !i64 ):
+  %1 = "llvm.add" (%0, %0) : (!i64, !i64 ) -> (!i64)
+  "return" (%1) : ( !i64) -> ()
+}], rhs := [_| {
+  ^entry (%0: !r64 ):
+  %1 = "add" (%0, %0) : (!r64, !r64 ) -> (!r64)
+  "return" (%1) : ( !r64) -> ()
+}], correct := by sorry }
+
+
+
+
+
+-- test if the intra dialect lowering works
+def testAddLowering : loweringLLVMtoRISCV exampleLLVM1 = some (exampleRiscv1) := by native_decide
+/-
+ rhs:=
 [_| {
   ^entry (%0: !r64 ):
   %1 = "add" (%0, %0) : (!r64, !r64 ) -> (!r64)
@@ -266,4 +707,5 @@ def loweringViaRewriter :  PeepholeRewrite llvm.riscv ([Ty.opt64]) .bv64 :=
 }], correct := by sorry }
 
 
-def testAddLowering : loweringLLVMtoRISCV exampleLLVM1 = some (exampleRiscv1) := by native_decide
+
+-/
