RiscvDialect.lean
@@ -2,3 +2,7 @@
 -- import RiscvDialect.Dialect
 
 import SSA.Core.Framework
+
+
+def main : IO Unit :=
+  IO.println "Hello from RiscvDialect!"
