RiscvDialect/Peephole_Optimizations/RiscVRefinement.lean
@@ -4,7 +4,7 @@ import SSA.Core.ErasedContext
 import SSA.Core.HVector
 import SSA.Core.EffectKind
 import SSA.Core.Util
-import RiscvDialect.RDialect
+-- import RiscvDialect.RDialect
 import SSA.Projects.InstCombine.LLVM.PrettyEDSL
 --import SSA.Projects.InstCombine.Refinement
 import SSA.Projects.InstCombine.Tactic
@@ -20,9 +20,11 @@ import SSA.Core.MLIRSyntax.GenericParser
 import SSA.Core.MLIRSyntax.EDSL
 import SSA.Projects.InstCombine.Tactic
 import Mathlib.Tactic.Ring
+import RiscvDialect.RISCV64.Syntax
+import RiscvDialect.RISCV64.Base
+import RiscvDialect.RISCV64.Semantics
 
-open RV64
-open toRISCV -- the riscv dialect
+open RISCV64 -- acces the RISCV64 dialect namespace
 
 def RiscvInstrSeqRefines (x y : BitVec 64) : Prop := x = y
 -- target is a refinement of source
@@ -32,6 +34,5 @@ infix:50 (priority:=low) " ⊑ᵣ" => RiscvInstrSeqRefines
 abbrev Com.RefinementRiscv (src tgt : Com RV64 Γ .pure t)
     (h : RV64TyDenote.toType t = BitVec 64 := by rfl) : Prop :=
   ∀ Γv, (h ▸ src.denote Γv) ⊑ᵣ (h ▸ tgt.denote Γv) -- in they end they must yield the same register value
-
 
 infixr:90 " ⊑ᵣ"  => Com.RefinementRiscv --applies this function so just an infix operator
