RiscvDialect/RISCV64/Base.lean
@@ -1,0 +1,366 @@
+
+import RiscvDialect.RISCV64.Semantics
+import SSA.Core.Framework
+set_option maxHeartbeats 1000000000000000000
+
+open RV64Semantics /- access the semantics -/
+
+namespace RISCV64
+/-! ## The `RISCV64` dialect -/
+/-!
+## Dialect operation definitions
+Modelled operations such that their inputs arguments are up to two register content values. Any other attributes e.g flags
+are encoded as part of the op-code.
+
+ Modells base ISA & ZBA/ZBB extension instructions.
+-/
+inductive Op
+|const : (val : Int) → Op -- const is not part of the RISC-V ISA but is used to in this dialect to modell immediates.
+|addiw (imm : BitVec 12) -- TO DO: rethink this design
+|lui (imm : BitVec 20)
+|auipc (imm : BitVec 20)
+|slliw (shamt : BitVec 5)
+|srliw (shamt : BitVec 5)
+|sraiw (shamt : BitVec 5)
+|slli (shamt : BitVec 6)
+|srli (shamt : BitVec 6)
+|srai (shamt : BitVec 6)
+|addw
+|subw
+|sllw
+|srlw
+|sraw
+|add
+|slt
+|sltu
+|and
+|or
+|xor
+|sll
+|srl
+|sub
+|sra
+|remw
+|rem
+|mul
+|mulu
+|mulw
+|mulh
+|mulhu
+|mulhsu
+|divu
+|rol
+|ror
+|remwu
+|remu
+ --the sign or unsigned when calling the function -> pattern match on to mul op to get the correct cases
+|divw
+|divwu
+|div
+|addi (imm : BitVec 12)
+|slti (imm : BitVec 12)
+|sltiu (imm : BitVec 12)
+|andi (imm : BitVec 12)
+|ori (imm : BitVec 12)
+|xori (imm : BitVec 12)
+|czero.eqz
+|czero.nez
+|bclr
+|bext
+|binv
+|bset
+|bclri (shamt : BitVec 6)
+|bexti (shamt : BitVec 6)
+|binvi (shamt : BitVec 6)
+|bseti (shamt : BitVec 6)
+|sext.b
+|sext.h
+|zext.h
+|rolw
+|rorw
+/-
+|pack
+|packh
+-- TO DO zbb_rytpe full
+|add.uw
+|sh1add.uw
+|sh2add.uw
+|sh3add.uw
+|sh1add
+|sh2add
+|sh3add -/
+deriving DecidableEq, Repr
+
+
+/--
+## Dialect type definitions
+Defining a type system for the `RISCV64` dialect. `bv` represents bit vector.
+-/
+inductive Ty
+  | bv : Ty
+  deriving DecidableEq, Repr
+
+/-!
+Connecting the `bv` type to its underlying Lean type `BitVec 64`. By providing a `TyDenote` instance,
+we define how the `RISCV64` types transalte into actual Lean types.
+-/
+open TyDenote (toType) in
+instance RV64TyDenote : TyDenote Ty where
+toType := fun
+| Ty.bv => BitVec 64
+
+/--
+Provding a default instance for `bv`, which is a 64-bit zero bit vector.
+-/
+instance : Inhabited (TyDenote.toType (t : Ty)) where
+  default := by
+    cases t
+    exact (0#64)
+
+
+/--
+## Dialect operation definitions
+
+Specifing the signature of each `RISCV64` operation. `Sig` refers to the input types
+for each operation as a list of types.
+
+We mark it as `simp` and `reducible` such that the type checker and elaborator
+always fully unfold an `sig` to its underlying defintion and when the simplifier
+encounters a `sig` it can replace it by its definition.
+-/
+
+@[simp, reducible]
+def Op.sig : Op → List Ty
+  |.const _ =>  []
+  |.mulu  => [Ty.bv, Ty.bv]
+  |mulh  => [Ty.bv, Ty.bv]
+  |mulhu  => [Ty.bv, Ty.bv]
+  |mulhsu  => [Ty.bv, Ty.bv]
+  |divu =>  [Ty.bv, Ty.bv]
+  |rol => [Ty.bv, Ty.bv]
+  |ror => [Ty.bv, Ty.bv]
+  |.remwu  => [Ty.bv, Ty.bv]
+  |.remu  =>  [Ty.bv, Ty.bv]
+  |.addiw (imm : BitVec 12) => [Ty.bv]
+  |.lui (imm : BitVec 20) => [Ty.bv]
+  |.auipc (imm : BitVec 20)  => [Ty.bv]
+  |.slliw (shamt : BitVec 5)  => [Ty.bv]
+  |.srliw (shamt : BitVec 5) => [Ty.bv]
+  |.sraiw (shamt : BitVec 5) => [Ty.bv]
+  |.slli (shamt : BitVec 6) => [Ty.bv]
+  |.srli (shamt : BitVec 6) => [Ty.bv]
+  |srai (shamt : BitVec 6) => [Ty.bv]
+  |.addw => [Ty.bv, Ty.bv]
+  |.subw => [Ty.bv, Ty.bv]
+  |.sllw => [Ty.bv, Ty.bv]
+  |.srlw => [Ty.bv, Ty.bv]
+  |.sraw => [Ty.bv, Ty.bv]
+  |.add => [Ty.bv, Ty.bv]
+  |.slt => [Ty.bv, Ty.bv]
+  |.sltu => [Ty.bv, Ty.bv]
+  |.and => [Ty.bv, Ty.bv]
+  |.or => [Ty.bv, Ty.bv]
+  |.xor => [Ty.bv, Ty.bv]
+  |.sll => [Ty.bv, Ty.bv]
+  |.srl => [Ty.bv, Ty.bv]
+  |.sub => [Ty.bv, Ty.bv]
+  |.sra => [Ty.bv, Ty.bv]
+  |.remw  => [Ty.bv, Ty.bv]
+  |.rem  =>  [Ty.bv, Ty.bv]
+  |.mul => [Ty.bv, Ty.bv]
+  |.mulw => [Ty.bv, Ty.bv]
+  |.div  =>  [Ty.bv, Ty.bv]
+  |.divw  =>  [Ty.bv, Ty.bv]
+  |.divwu  =>  [Ty.bv, Ty.bv]
+  |.addi (imm : BitVec 12) => [Ty.bv]
+  |.slti (imm : BitVec 12) => [Ty.bv]
+  |.sltiu (imm : BitVec 12) => [Ty.bv]
+  |.andi (imm : BitVec 12) => [Ty.bv]
+  |.ori (imm : BitVec 12) => [Ty.bv]
+  |.xori (imm : BitVec 12) => [Ty.bv]
+  |.czero.eqz =>  [Ty.bv, Ty.bv]
+  |.czero.nez =>  [Ty.bv, Ty.bv]
+  |.sext.b => [Ty.bv]
+  |.sext.h => [Ty.bv]
+  |.zext.h => [Ty.bv]
+  |bclr => [Ty.bv, Ty.bv]
+  |bext => [Ty.bv, Ty.bv]
+  |binv => [Ty.bv, Ty.bv]
+  |bset  => [Ty.bv, Ty.bv]
+  |bclri (shamt : BitVec 6) => [Ty.bv]
+  |bexti (shamt : BitVec 6) => [Ty.bv]
+  |binvi (shamt : BitVec 6) => [Ty.bv]
+  |bseti (shamt : BitVec 6) => [Ty.bv]
+  |rolw => [Ty.bv, Ty.bv]
+  |rorw => [Ty.bv, Ty.bv]
+
+
+/--
+Specifing the `outTy` of each `RISCV64` operation.
+Again, we mark  it as `simp` and `reducible`.
+-/
+
+@[simp, reducible]
+def Op.outTy : Op  → Ty
+  |.const _ => Ty.bv
+  |.mulu  => Ty.bv
+  |.mulh  => Ty.bv
+  |.mulhu  => Ty.bv
+  |.mulhsu  => Ty.bv
+  |.divu =>  Ty.bv
+  |.rol => Ty.bv
+  |.ror => Ty.bv
+  |.remwu  => Ty.bv
+  |.remu  =>  Ty.bv
+  |.addiw (imm : BitVec 12) => Ty.bv
+  |.lui (imm : BitVec 20) => Ty.bv
+  |.auipc (imm : BitVec 20) => Ty.bv
+  |.slliw (shamt : BitVec 5) => Ty.bv
+  |.srliw (shamt : BitVec 5) => Ty.bv
+  |.sraiw (shamt : BitVec 5) => Ty.bv
+  |.slli (shamt : BitVec 6) => Ty.bv
+  |.srli (shamt : BitVec 6) => Ty.bv
+  |srai (shamt : BitVec 6) => Ty.bv
+  |.addw => Ty.bv
+  |.subw => Ty.bv
+  |.sllw => Ty.bv
+  |.srlw => Ty.bv
+  |.sraw => Ty.bv
+  |.add => Ty.bv
+  |.slt => Ty.bv
+  |.sltu => Ty.bv
+  |.and => Ty.bv
+  |.or => Ty.bv
+  |.xor => Ty.bv
+  |.sll => Ty.bv
+  |.srl => Ty.bv
+  |.sub => Ty.bv
+  |.sra => Ty.bv
+  |.remw  => Ty.bv
+  |.rem =>  Ty.bv
+  |.mul => Ty.bv
+  |.mulw => Ty.bv
+  |.div=>  Ty.bv
+  |.divw  =>  Ty.bv
+  |.divwu  =>  Ty.bv
+  |.addi (imm : BitVec 12) => Ty.bv
+  |.slti (imm : BitVec 12) => Ty.bv
+  |.sltiu (imm : BitVec 12) => Ty.bv
+  |.andi (imm : BitVec 12) => Ty.bv
+  |.ori (imm : BitVec 12) => Ty.bv
+  |.xori (imm : BitVec 12) => Ty.bv
+  |.czero.eqz =>   Ty.bv
+  |.czero.nez =>  Ty.bv
+  |.sext.b => Ty.bv
+  |.sext.h => Ty.bv
+  |.zext.h => Ty.bv
+  |bclr => Ty.bv
+  |bext => Ty.bv
+  |binv => Ty.bv
+  |bset  => Ty.bv
+  |bclri (shamt : BitVec 6) => Ty.bv
+  |bexti (shamt : BitVec 6) => Ty.bv
+  |binvi (shamt : BitVec 6) => Ty.bv
+  |bseti (shamt : BitVec 6) => Ty.bv
+  |rolw => Ty.bv
+  |rorw => Ty.bv
+
+
+/-- Combine `outTy` and `sig` together into a `Signature`. -/
+@[simp, reducible]
+def Op.signature : Op → Signature (Ty) :=
+  fun o => {sig := Op.sig o, outTy := Op.outTy o, regSig := []} --ASK what is meant by regSig ?
+
+
+
+/--
+Bundling the `Ops`and `Ty`into a dialect and abbreviating `RISCV64` into a dialect named `RV64`.
+We pass our `Op.signature` as an instance -/
+abbrev RV64 : Dialect where
+  Op := Op
+  Ty := Ty
+
+instance : DialectSignature RV64 := ⟨Op.signature⟩
+
+-- DEBUG: only addapted the get0 get1 of the instruction that where used in the insteuction selcetion so far, to be extended
+-- I assume the layout is add (then all the args in the op code) (then args in the signature) ret_val
+
+/--
+## Dialect semantics
+
+We assign semantics defined in `RV64` to each operation. This defines the meaning of each operation in Lean.
+
+When writting RISC-V-like abstract MLIR ISA intutivly we write `op  arg1 arg2`. The `RISCV64` are defined to
+first process the second operand then the first. Therefore we first pass `.get 1` then `.get 0` into the
+functions that define our semantics.
+-/
+@[simp, reducible]
+instance : DialectDenote (RV64) where
+  denote
+  |.const val,_,  _  => BitVec.ofInt 64 val
+  |.addiw imm, regs, _   => ADDIW_pure64 imm (regs.getN 0 (by simp [DialectSignature.sig, signature]))
+  |.lui imm,  regs , _   => UTYPE_pure64_lui imm (regs.getN 0 (by simp [DialectSignature.sig, signature]))
+  |.auipc imm, regs, _  => UTYPE_pure64_AUIPC imm (regs.getN 0 (by simp [DialectSignature.sig, signature]))
+  |.slliw shamt, regs, _  => SHIFTIWOP_pure64_RISCV_SLLIW shamt (regs.getN 0 (by simp [DialectSignature.sig, signature]))
+  |.srliw shamt, regs, _  => SHIFTIWOP_pure64_RISCV_SRLIW shamt (regs.getN 0 (by simp [DialectSignature.sig, signature]))
+  |.sraiw shamt, regs, _  => SHIFTIWOP_pure64_RISCV_SRAIW shamt (regs.getN 0 (by simp [DialectSignature.sig, signature]))
+  |.slli shamt, regs, _  => SHIFTIOP_pure64_RISCV_SLLI shamt (regs.getN 0 (by simp [DialectSignature.sig, signature]))
+  |.srli shamt, regs, _  => SHIFTIOP_pure64_RISCV_SRLI shamt (regs.getN 0 (by simp [DialectSignature.sig, signature]))
+  |.srai shamt, regs, _  => SHIFTIOP_pure64_RISCV_SRAI shamt  (regs.getN 0 (by simp [DialectSignature.sig, signature]))
+  |.addw, regs, _  =>  RTYPEW_pure64_RISCV_ADDW (regs.getN 0 (by simp [DialectSignature.sig, signature]))  (regs.getN 1 (by simp [DialectSignature.sig, signature]))
+  |.subw, regs, _  => RTYPEW_pure64_RISCV_SUBW (regs.getN 0 (by simp [DialectSignature.sig, signature]))  (regs.getN 1 (by simp [DialectSignature.sig, signature]))
+  |.sllw, regs, _  => RTYPEW_pure64_RISCV_SLLW (regs.getN 0 (by simp [DialectSignature.sig, signature]))  (regs.getN 1 (by simp [DialectSignature.sig, signature]))
+  |.srlw, regs, _  => RTYPEW_pure64_RISCV_SRLW (regs.getN 0 (by simp [DialectSignature.sig, signature]))  (regs.getN 1 (by simp [DialectSignature.sig, signature]))
+  |.sraw, regs, _ => RTYPEW_pure64_RISCV_SRAW (regs.getN 0 (by simp [DialectSignature.sig, signature]))  (regs.getN 1 (by simp [DialectSignature.sig, signature]))
+  |.add, regs, _ => RTYPE_pure64_RISCV_ADD (regs.getN 0 (by simp [DialectSignature.sig, signature]))  (regs.getN 1 (by simp [DialectSignature.sig, signature]))
+  |.slt, regs, _ => RTYPE_pure64_RISCV_SLT (regs.getN 0 (by simp [DialectSignature.sig, signature]))  (regs.getN 1 (by simp [DialectSignature.sig, signature]))
+  |.sltu, regs, _ => RTYPE_pure64_RISCV_SLTU (regs.getN 0 (by simp [DialectSignature.sig, signature]))  (regs.getN 1 (by simp [DialectSignature.sig, signature]))
+  |.and, regs, _ => RTYPE_pure64_RISCV_AND (regs.getN 0 (by simp [DialectSignature.sig, signature]))  (regs.getN 1 (by simp [DialectSignature.sig, signature]))
+  |.or, regs, _ => RTYPE_pure64_RISCV_OR (regs.getN 0 (by simp [DialectSignature.sig, signature]))  (regs.getN 1 (by simp [DialectSignature.sig, signature]))
+  |.xor, regs, _ => RTYPE_pure64_RISCV_XOR (regs.getN 0 (by simp [DialectSignature.sig, signature]))  (regs.getN 1 (by simp [DialectSignature.sig, signature]))
+  |.sll, regs, _ => RTYPE_pure64_RISCV_SLL (regs.getN 1 (by simp [DialectSignature.sig, signature]))  (regs.getN 0 (by simp [DialectSignature.sig, signature]))
+  |.srl, regs, _ => RTYPE_pure64_RISCV_SRL (regs.getN 1 (by simp [DialectSignature.sig, signature]))  (regs.getN 0 (by simp [DialectSignature.sig, signature]))
+  |.sub, regs, _  => RTYPE_pure64_RISCV_SUB (regs.getN 0 (by simp [DialectSignature.sig, signature]))  (regs.getN 1 (by simp [DialectSignature.sig, signature]))
+  |.sra, regs, _  => RTYPE_pure64_RISCV_SRA (regs.getN 1 (by simp [DialectSignature.sig, signature]))  (regs.getN 0 (by simp [DialectSignature.sig, signature]))
+  |.remw, regs, _  => REMW_pure64_signed (regs.getN 0 (by simp [DialectSignature.sig, signature]))  (regs.getN 1 (by simp [DialectSignature.sig, signature]))-- double-check
+  |.remwu, regs, _  => REMW_pure64_unsigned (regs.getN 0 (by simp [DialectSignature.sig, signature]))  (regs.getN 1 (by simp [DialectSignature.sig, signature]))-- double-check
+  |.rem, regs, _  =>  REM_pure64_signed (regs.getN 1 (by simp [DialectSignature.sig, signature]))  (regs.getN 0 (by simp [DialectSignature.sig, signature]))
+  |.remu, regs, _ =>  REM_pure64_unsigned (regs.getN 1 (by simp [DialectSignature.sig, signature]))  (regs.getN 0 (by simp [DialectSignature.sig, signature]))
+  |.mulu, regs, _ => MUL_pure64_fff (regs.getN 0 (by simp [DialectSignature.sig, signature]))  (regs.getN 1 (by simp [DialectSignature.sig, signature])) -- double check
+  --|.mul false false true , regs, _ => RV64.MUL_pure64_fft (regs.getN 0 (by simp [DialectSignature.sig, signature]))  (regs.getN 1 (by simp [DialectSignature.sig, signature]))
+  --|.mul  false true false , regs, _ => RV64.MUL_pure64_ftf (regs.getN 0 (by simp [DialectSignature.sig, signature]))  (regs.getN 1 (by simp [DialectSignature.sig, signature]))
+  |.mulhu,regs, _ => MUL_pure64_tff (regs.getN 0 (by simp [DialectSignature.sig, signature]))  (regs.getN 1 (by simp [DialectSignature.sig, signature]))
+  |.mul ,regs, _ => MUL_pure64_ftt (regs.getN 0 (by simp [DialectSignature.sig, signature]))  (regs.getN 1 (by simp [DialectSignature.sig, signature]))
+  --|.mul  true false true,regs, _ => RV64.MUL_pure64_tft (regs.getN 0 (by simp [DialectSignature.sig, signature]))  (regs.getN 1 (by simp [DialectSignature.sig, signature]))
+  |.mulhsu ,regs, _ => MUL_pure64_ttf (regs.getN 0 (by simp [DialectSignature.sig, signature]))  (regs.getN 1 (by simp [DialectSignature.sig, signature]))
+  |.mulh,regs, _ => MUL_pure64_ttt (regs.getN 0 (by simp [DialectSignature.sig, signature]))  (regs.getN 1 (by simp [DialectSignature.sig, signature]))
+  |.mulw,  regs, _ => MULW_pure64 (regs.getN 0 (by simp [DialectSignature.sig, signature]))  (regs.getN 1 (by simp [DialectSignature.sig, signature])) -- double check
+  |.div, regs, _  =>  DIV_pure64_signed (regs.getN 1 (by simp [DialectSignature.sig, signature]))  (regs.getN 0 (by simp [DialectSignature.sig, signature]))
+  |.divu,  regs, _ =>  DIV_pure64_unsigned (regs.getN 0 (by simp [DialectSignature.sig, signature]))  (regs.getN 1 (by simp [DialectSignature.sig, signature]))
+  |.divw, regs, _  =>  DIVW_pure64_signed (regs.getN 0 (by simp [DialectSignature.sig, signature]))  (regs.getN 1 (by simp [DialectSignature.sig, signature]))
+  |.divwu, regs, _ =>  DIVW_pure64_unsigned (regs.getN 0 (by simp [DialectSignature.sig, signature]))  (regs.getN 1 (by simp [DialectSignature.sig, signature]))
+  |.addi imm, reg, _  => ITYPE_pure64_RISCV_ADDI  imm (reg.getN 0 (by simp [DialectSignature.sig, signature]))
+  |.slti imm, reg, _  => ITYPE_pure64_RISCV_SLTI  imm (reg.getN 0 (by simp [DialectSignature.sig, signature]))
+  |.sltiu imm, reg, _ => ITYPE_pure64_RISCV_SLTIU  imm (reg.getN 0 (by simp [DialectSignature.sig, signature]))
+  |.andi imm, reg, _=> ITYPE_pure64_RISCV_ANDI  imm (reg.getN 0 (by simp [DialectSignature.sig, signature]))
+  |.ori imm, reg, _ => ITYPE_pure64_RISCV_ORI  imm (reg.getN 0 (by simp [DialectSignature.sig, signature]))
+  |.xori imm, reg, _=> ITYPE_pure64_RISCV_XORI  imm (reg.getN 0 (by simp [DialectSignature.sig, signature]))
+  |.czero.eqz, regs, _ => ZICOND_RTYPE_pure64_RISCV_CZERO_EQZ (regs.getN 0 (by simp [DialectSignature.sig, signature]))  (regs.getN 1 (by simp [DialectSignature.sig, signature]))
+  |.czero.nez, regs, _ => ZICOND_RTYPE_pure64_RISCV_RISCV_CZERO_NEZ (regs.getN 0 (by simp [DialectSignature.sig, signature]))  (regs.getN 1 (by simp [DialectSignature.sig, signature]))
+  |.sext.b, reg, _ => ZBB_EXTOP_pure64_RISCV_SEXTB (reg.getN 0 (by simp [DialectSignature.sig, signature]))
+  |.sext.h, reg, _ => ZBB_EXTOP_pure64_RISCV_SEXTH (reg.getN 0 (by simp [DialectSignature.sig, signature]))
+  |.zext.h, reg, _ => ZBB_EXTOP_pure64_RISCV_ZEXTH (reg.getN 0 (by simp [DialectSignature.sig, signature]))
+  |.bclr, regs, _  => ZBS_RTYPE_pure64_RISCV_BCLR (regs.getN 0 (by simp [DialectSignature.sig, signature]))  (regs.getN 1 (by simp [DialectSignature.sig, signature]))
+  |.bext, regs, _  => ZBS_RTYPE_pure64_RISCV_BEXT (regs.getN 0 (by simp [DialectSignature.sig, signature]))  (regs.getN 1 (by simp [DialectSignature.sig, signature]))
+  |.binv, regs, _  => ZBS_RTYPE_pure64_BINV (regs.getN 0 (by simp [DialectSignature.sig, signature]))  (regs.getN 1 (by simp [DialectSignature.sig, signature]))
+  |.bset, regs, _   => ZBS_RTYPE_pure64_RISCV_BSET (regs.getN 0 (by simp [DialectSignature.sig, signature]))  (regs.getN 1 (by simp [DialectSignature.sig, signature]))
+  |.bclri shamt , reg, _  => ZBS_IOP_pure64_RISCV_BCLRI (shamt) (reg.getN 0 (by simp [DialectSignature.sig, signature]))
+  |.bexti shamt, reg, _  => ZBS_IOP_pure64_RISCV_BEXTI (shamt) (reg.getN 0 (by simp [DialectSignature.sig, signature]))
+  |.binvi shamt, reg, _ => ZBS_IOP_pure64_RISCV_BINVI (shamt) (reg.getN 0 (by simp [DialectSignature.sig, signature]))
+  |.bseti shamt, reg, _ => ZBS_IOP_pure64_RISCV_BSETI (shamt) (reg.getN 0 (by simp [DialectSignature.sig, signature]))
+  |.rolw, regs, _ => ZBB_RTYPEW_pure64_RISCV_ROLW (regs.getN 0 (by simp [DialectSignature.sig, signature]))  (regs.getN 1 (by simp [DialectSignature.sig, signature]))
+  |.rorw, regs, _ => ZBB_RTYPEW_pure64_RISCV_RORW (regs.getN 0 (by simp [DialectSignature.sig, signature]))  (regs.getN 1 (by simp [DialectSignature.sig, signature]))
+  |.rol, regs, _ => ZBB_RTYPE_pure64_RISCV_ROL (regs.getN 0 (by simp [DialectSignature.sig, signature]))  (regs.getN 1 (by simp [DialectSignature.sig, signature]))
+  |.ror, regs, _ => ZBB_RTYPE_pure64_RISCV_ROR (regs.getN 0 (by simp [DialectSignature.sig, signature]))  (regs.getN 1 (by simp [DialectSignature.sig, signature]))
+
+end RISCV64
