RiscvDialect/RISCV64/Semantics.lean
@@ -1,0 +1,366 @@
+import SSA.Core.MLIRSyntax.EDSL
+set_option maxHeartbeats 1000000000000000000
+
+/-!
+  ## Dialect semantics
+  Every ISA instruction is modelled to operate on 64-bit bit vectors only.
+  This should allow to gain in automation using the bv_decide.
+-/
+
+namespace RV64Semantics
+
+def ADDIW_pure64 (imm : BitVec 12) (rs1_val : BitVec 64) :  BitVec 64 :=
+     BitVec.signExtend 64 (BitVec.setWidth 32 (BitVec.add (BitVec.signExtend 64 imm) rs1_val))
+
+-- loads immediate into upper 20 bits and then fills the rest up with 0 and returns it as the result
+def UTYPE_pure64_lui (imm : BitVec 20) (pc : BitVec 64) : BitVec 64 :=
+     BitVec.signExtend 64 (imm ++ (0x000 : (BitVec 12)))
+
+-- loads immediate into upper 20 bits and then fills the rest up with 0 and returns, adds the program counter and then returns it as a result
+def UTYPE_pure64_AUIPC (imm : BitVec 20) (pc : BitVec 64)  : BitVec 64 :=
+    BitVec.add (BitVec.signExtend 64 (BitVec.append imm (0x000 : (BitVec 12)))) pc
+
+def SHIFTIWOP_pure64_RISCV_SLLIW (shamt : BitVec 5) (rs1_val : BitVec 64) : BitVec 64 :=
+    BitVec.signExtend 64 (BitVec.shiftLeft (BitVec.extractLsb' 0 32 rs1_val) (shamt).toNat)
+
+-- logical rightshift, filled with zeros x/2^s rounding down
+def SHIFTIWOP_pure64_RISCV_SRLIW (shamt : BitVec 5) (rs1_val : BitVec 64) : BitVec 64 :=
+    BitVec.signExtend 64 (BitVec.ushiftRight (BitVec.extractLsb' 0 32 rs1_val) (shamt).toNat)
+
+
+def SHIFTIWOP_pure64_RISCV_SRAIW (shamt : BitVec 5) (rs1_val : BitVec 64) : BitVec 64
+    :=
+    BitVec.signExtend 64
+      (BitVec.setWidth 32
+       (BitVec.extractLsb
+         (31 + shamt.toNat)
+          shamt.toNat
+          (BitVec.signExtend ((32) + shamt.toNat) (BitVec.extractLsb 31 0 rs1_val))
+        )
+      )
+
+def SHIFTIOP_pure64_RISCV_SLLI (shamt : BitVec 6) (rs1_val : BitVec 64)  : BitVec 64
+    := BitVec.shiftLeft rs1_val shamt.toNat
+
+def SHIFTIOP_pure64_RISCV_SRLI (shamt : BitVec 6) (rs1_val : BitVec 64) : BitVec 64 :=
+    BitVec.ushiftRight rs1_val shamt.toNat
+
+-- here I didnt specify a return type bc it depends
+def SHIFTIOP_pure64_RISCV_SRAI (shamt : (BitVec 6)) (rs1_val : (BitVec 64)): BitVec 64 :=
+    let value := rs1_val ;
+    let shift := shamt.toNat;
+    BitVec.setWidth 64 (BitVec.extractLsb (63 + shift) shift (BitVec.signExtend (64 + shift) value)) -- had to this to tell lean how to hanlde the type
+   -- (BitVec.extractLsb (63 + shift)  shift  (BitVec.signExtend ((64 + shift)) value) : BitVec 64)
+
+-- simple integer operations on 32-bit word and then sign extend result to 64 bits
+def RTYPEW_pure64_RISCV_ADDW (rs2_val : BitVec 64) (rs1_val : BitVec 64) : BitVec 64 :=
+      let rs1_val32 := BitVec.extractLsb' 0 32 rs1_val;
+      let rs2_val32 := BitVec.extractLsb' 0 32 rs2_val;
+      BitVec.signExtend 64 (BitVec.add rs1_val32 rs2_val32)
+
+def RTYPEW_pure64_RISCV_SUBW (rs2_val : BitVec 64) (rs1_val : BitVec 64) : BitVec 64 :=
+      let rs1_val32 := BitVec.extractLsb' 0 32 rs1_val;
+      let rs2_val32 := BitVec.extractLsb' 0 32 rs2_val;
+      BitVec.signExtend 64 (BitVec.sub rs1_val32 rs2_val32)
+
+-- can be all done by rfl
+def RTYPEW_pure64_RISCV_SLLW (rs2_val : BitVec 64) (rs1_val : BitVec 64) : BitVec 64 :=
+    let rs1_val32 := BitVec.extractLsb' 0 32 rs1_val;
+    let rs2_val32 := BitVec.extractLsb' 0 32 rs2_val;
+    let shamt := BitVec.extractLsb' 0 5 rs2_val32;
+    BitVec.signExtend 64 (BitVec.shiftLeft rs1_val32 shamt.toNat)
+
+-- can be all done by rfl
+def RTYPEW_pure64_RISCV_SRLW (rs2_val : BitVec 64) (rs1_val : BitVec 64)  : BitVec 64 :=
+    let rs1_val32 := BitVec.extractLsb' 0 32 rs1_val;
+    let rs2_val32 := BitVec.extractLsb' 0 32 rs2_val;
+    let shamt := BitVec.extractLsb' 0 5 rs2_val32;
+    BitVec.signExtend 64 (BitVec.ushiftRight rs1_val32 shamt.toNat)
+
+def RTYPEW_pure64_RISCV_SRAW (rs2_val : (BitVec 64)) (rs1_val : (BitVec 64)) :=
+BitVec.signExtend 64
+           (BitVec.setWidth 32
+              (BitVec.extractLsb
+                 (31 + rs2_val.toNat % 4294967296 % 32)
+                     (rs2_val.toNat % 4294967296 % 32)
+                          (BitVec.signExtend (32 + rs2_val.toNat % 4294967296 % 32)
+                              (BitVec.extractLsb 31 0 rs1_val))))
+
+
+def RTYPE_pure64_RISCV_ADD (rs2_val : BitVec 64) (rs1_val : BitVec 64) :BitVec 64 :=
+      BitVec.add rs1_val rs2_val
+
+def RTYPE_pure64_RISCV_SLT (rs2_val : BitVec 64) (rs1_val : BitVec 64) : BitVec 64 :=
+    let b := BitVec.slt rs1_val rs2_val;
+    BitVec.setWidth 64 (BitVec.ofBool b)
+
+def RTYPE_pure64_RISCV_SLTU (rs2_val : BitVec 64) (rs1_val : BitVec 64) : BitVec 64 :=
+    let b := BitVec.ult rs1_val rs2_val;
+      BitVec.setWidth 64 (BitVec.ofBool b)
+
+def RTYPE_pure64_RISCV_AND (rs2_val : BitVec 64) (rs1_val : BitVec 64) : BitVec 64 :=
+      BitVec.and rs2_val rs1_val
+
+def RTYPE_pure64_RISCV_OR(rs2_val : BitVec 64) (rs1_val : BitVec 64) : BitVec 64 :=
+      BitVec.or rs2_val rs1_val
+
+def RTYPE_pure64_RISCV_XOR(rs2_val : BitVec 64) (rs1_val : BitVec 64) : BitVec 64 :=
+      BitVec.xor rs2_val rs1_val
+
+def RTYPE_pure64_RISCV_SLL (rs2_val : BitVec 64) (rs1_val : BitVec 64) : BitVec 64 :=
+       let shamt := (BitVec.extractLsb 5 0 rs2_val).toNat;
+       BitVec.shiftLeft rs1_val shamt
+
+def RTYPE_pure64_RISCV_SRL (rs2_val : BitVec 64) (rs1_val : BitVec 64) : BitVec 64 :=
+      let shamt := (BitVec.extractLsb 5 0 rs2_val).toNat;
+      BitVec.ushiftRight rs1_val shamt
+
+def RTYPE_pure64_RISCV_SUB (rs2_val : BitVec 64) (rs1_val : BitVec 64) : BitVec 64 :=
+    BitVec.sub rs1_val rs2_val
+
+def RTYPE_pure64_RISCV_SRA (rs2_val : BitVec 64) (rs1_val : BitVec 64) :=
+BitVec.setWidth 64
+      (BitVec.extractLsb
+        (63 + (BitVec.extractLsb 5 0 rs2_val).toNat)
+        (BitVec.extractLsb 5 0 rs2_val).toNat
+        (BitVec.signExtend
+          (64 + (BitVec.extractLsb 5 0 rs2_val).toNat) rs1_val))
+
+
+def REMW_pure64_unsigned (rs2_val : BitVec 64) (rs1_val : BitVec 64): BitVec 64 :=
+  BitVec.signExtend 64
+    (BitVec.extractLsb' 0 32
+      (BitVec.ofInt 33
+        (Int.ofNat
+          (if Int.ofNat (BitVec.extractLsb 31 0 rs2_val).toNat = 0 then Int.ofNat (BitVec.extractLsb 31 0 rs1_val).toNat
+            else
+              (Int.ofNat (BitVec.extractLsb 31 0 rs1_val).toNat).tmod
+                (Int.ofNat (BitVec.extractLsb 31 0 rs2_val).toNat)).toNat)))
+
+def REMW_pure64_signed (rs2_val : (BitVec 64)) (rs1_val : (BitVec 64)) : BitVec 64 :=
+    BitVec.signExtend 64
+    (BitVec.extractLsb' 0 32
+      (BitVec.ofInt 33
+        (Int.ofNat
+          (if (BitVec.extractLsb 31 0 rs2_val).toInt = 0 then (BitVec.extractLsb 31 0 rs1_val).toInt
+            else (BitVec.extractLsb 31 0 rs1_val).toInt.tmod (BitVec.extractLsb 31 0 rs2_val).toInt).toNat)))
+
+--    PureFunctions.execute_REM_pure64 (False) rs2_val rs1_val  important to set sign bit to false
+def REM_pure64_unsigned (rs2_val : BitVec 64) (rs1_val : BitVec 64) : BitVec 64  :=
+   BitVec.extractLsb' 0 64
+    (BitVec.ofInt 65
+      (Int.ofNat
+        (if Int.ofNat rs2_val.toNat = 0 then Int.ofNat rs1_val.toNat
+          else (Int.ofNat rs1_val.toNat).tmod (Int.ofNat rs2_val.toNat)).toNat))
+
+
+def REM_pure64_signed (rs2_val : BitVec 64) (rs1_val : BitVec 64) : BitVec 64  :=
+    BitVec.extractLsb' 0 64
+    (BitVec.ofInt 65
+      (Int.ofNat (if rs2_val.toInt = 0 then rs1_val.toInt else rs1_val.toInt.tmod rs2_val.toInt).toNat))
+
+
+def MULW_pure64 (rs2_val : (BitVec 64)) (rs1_val : (BitVec 64)) : BitVec 64 :=
+    BitVec.signExtend 64
+    (BitVec.extractLsb 31 0
+      (BitVec.extractLsb' 0 64
+        (BitVec.ofInt 65
+          ((BitVec.extractLsb 31 0 rs1_val).toInt * (BitVec.extractLsb 31 0 rs2_val).toInt).toNat)))
+
+def MUL_pure64_fff (rs2_val : BitVec 64) (rs1_val : BitVec 64) : BitVec 64 :=
+     BitVec.extractLsb 63 0
+        (BitVec.extractLsb' 0 128 (BitVec.ofInt 129 (max (Int.mul (Int.ofNat rs1_val.toNat) (Int.ofNat rs2_val.toNat)) 0)))
+
+
+def  MUL_pure64_fft (rs2_val : BitVec 64) (rs1_val : BitVec 64) : BitVec 64 :=
+  BitVec.extractLsb 63 0
+    (BitVec.extractLsb' 0 128
+      (BitVec.ofInt 129 (Int.ofNat (Int.mul (Int.ofNat rs1_val.toNat)  (rs2_val.toInt)).toNat)))
+
+#check BitVec.ofInt
+#check (Int.ofNat (Int.mul (BitVec.toInt 0#64) (Int.ofNat (BitVec.toNat 0#64))).toNat)
+
+def MUL_pure64_ftf (rs2_val : BitVec 64) (rs1_val : BitVec 64)  : BitVec 64 :=
+    BitVec.extractLsb 63 0
+      (BitVec.extractLsb' 0 128
+        (BitVec.ofInt 129
+        (Int.ofNat (Int.mul (BitVec.toInt rs1_val) (Int.ofNat (BitVec.toNat rs2_val))).toNat)))
+
+def MUL_pure64_tff (rs2_val : BitVec 64) (rs1_val : BitVec 64) : BitVec 64 :=
+    BitVec.extractLsb 127 64
+      (BitVec.extractLsb' 0 128
+        (BitVec.ofInt 129 (Int.ofNat (Int.mul (Int.ofNat rs1_val.toNat) (Int.ofNat rs2_val.toNat)).toNat)))
+
+
+def MUL_pure64_tft (rs2_val : BitVec 64) (rs1_val : BitVec 64) : BitVec 64 :=
+    BitVec.extractLsb 127 64
+    (BitVec.extractLsb' 0 128
+      (BitVec.ofInt 129 (Int.ofNat (Int.mul (Int.ofNat rs1_val.toNat) rs2_val.toInt).toNat)))
+
+
+def MUL_pure64_ttf (rs2_val : BitVec 64) (rs1_val : BitVec 64) : BitVec 64 :=
+  BitVec.extractLsb 127 64
+    (BitVec.extractLsb' 0 128
+      (BitVec.ofInt 129 (Int.ofNat (Int.mul rs1_val.toInt (Int.ofNat rs2_val.toNat)).toNat)))
+
+def MUL_pure64_ftt (rs2_val : BitVec 64) (rs1_val : BitVec 64) : BitVec 64 :=
+  BitVec.extractLsb 63 0
+    (BitVec.extractLsb' 0 128 (BitVec.ofInt 129 (Int.ofNat (Int.mul rs1_val.toInt rs2_val.toInt).toNat)))
+
+def MUL_pure64_ttt (rs2_val : BitVec 64) (rs1_val : BitVec 64) : BitVec 64 :=
+  BitVec.extractLsb 127 64
+    (BitVec.extractLsb' 0 128 (BitVec.ofInt 129 (Int.ofNat (Int.mul rs1_val.toInt rs2_val.toInt).toNat)))
+
+def DIVW_pure64_signed (rs2_val : BitVec 64) (rs1_val : BitVec 64) : BitVec 64 :=
+  BitVec.signExtend 64
+    (BitVec.extractLsb' 0 32
+      (BitVec.ofInt 33
+        (max
+          (if
+              2147483647 <
+                if (BitVec.extractLsb 31 0 rs2_val).toInt = 0 then -1
+                else (BitVec.extractLsb 31 0 rs1_val).toInt.tdiv (BitVec.extractLsb 31 0 rs2_val).toInt then
+            -2147483648
+          else
+            if (BitVec.extractLsb 31 0 rs2_val).toInt = 0 then -1
+            else (BitVec.extractLsb 31 0 rs1_val).toInt.tdiv (BitVec.extractLsb 31 0 rs2_val).toInt)
+          0)))
+
+def  DIVW_pure64_unsigned (rs2_val : BitVec 64) (rs1_val : BitVec 64) : BitVec 64 :=
+       BitVec.signExtend 64
+    (BitVec.extractLsb' 0 32
+      (BitVec.ofInt 33
+        (Int.ofNat
+          (if Int.ofNat (BitVec.extractLsb 31 0 rs2_val).toNat = 0 then -1
+            else
+              (Int.ofNat (BitVec.extractLsb 31 0 rs1_val).toNat).tdiv
+                (Int.ofNat (BitVec.extractLsb 31 0 rs2_val).toNat)).toNat)))
+
+def DIV_pure64_signed (rs2_val : BitVec 64) (rs1_val : BitVec 64) : BitVec 64 :=
+  BitVec.extractLsb' 0 64
+    (BitVec.ofInt 65
+      (max
+        (if 9223372036854775807 < if rs2_val.toInt = 0 then -1 else rs1_val.toInt.tdiv rs2_val.toInt then
+          -9223372036854775808
+        else if rs2_val.toInt = 0 then -1 else rs1_val.toInt.tdiv rs2_val.toInt)
+        0))
+
+def DIV_pure64_unsigned (rs2_val : BitVec 64) (rs1_val : BitVec 64) : BitVec 64 :=
+  BitVec.extractLsb' 0 64
+    (BitVec.ofNat 65
+      (if Int.ofNat rs2_val.toNat = 0 then -1 else (Int.ofNat rs1_val.toNat).tdiv (Int.ofNat rs2_val.toNat)).toNat)
+
+def ITYPE_pure64_RISCV_ADDI (imm : BitVec 12) (rs1_val : BitVec 64) : BitVec 64 :=
+    let immext : BitVec 64 := (BitVec.signExtend 64 imm) ;
+    BitVec.add rs1_val immext
+
+def ITYPE_pure64_RISCV_SLTI (imm : BitVec 12) (rs1_val : BitVec 64) : BitVec 64 :=
+       let immext : BitVec 64 := (BitVec.signExtend 64 imm);
+       let b := BitVec.slt rs1_val immext;
+       BitVec.zeroExtend 64 (BitVec.ofBool b)
+
+def ITYPE_pure64_RISCV_SLTIU (imm : BitVec 12) (rs1_val : BitVec 64) : BitVec 64 :=
+       let immext : BitVec 64 := (BitVec.signExtend 64 imm);
+       let b := BitVec.ult rs1_val immext;
+       BitVec.setWidth 64 (BitVec.ofBool b)
+
+def  ITYPE_pure64_RISCV_ANDI (imm : BitVec 12) (rs1_val : BitVec 64) : BitVec 64 :=
+    let immext : BitVec 64 := (BitVec.signExtend 64 imm);
+      BitVec.and rs1_val immext
+
+def ITYPE_pure64_RISCV_ORI (imm : BitVec 12) (rs1_val : BitVec 64) : BitVec 64 :=
+      let immext : BitVec 64 := (BitVec.signExtend 64 imm) ;
+      BitVec.or rs1_val immext
+
+
+def  ITYPE_pure64_RISCV_XORI (imm : (BitVec 12)) (rs1_val : (BitVec 64)) : BitVec 64 :=
+      let immext : BitVec 64 := (BitVec.signExtend 64 imm) ;
+      BitVec.xor rs1_val immext
+
+def ZICOND_RTYPE_pure64_RISCV_CZERO_EQZ (rs2_val : (BitVec 64)) (rs1_val : (BitVec 64)) :=
+      (if rs2_val = BitVec.zero 64 then BitVec.zero 64 else rs1_val)
+
+def ZICOND_RTYPE_pure64_RISCV_RISCV_CZERO_NEZ (rs2_val : (BitVec 64)) (rs1_val : (BitVec 64)) :=
+   (if rs2_val = BitVec.zero 64 then rs1_val else BitVec.zero 64)
+
+
+def ZBS_RTYPE_pure64_RISCV_BCLR (rs2_val : BitVec 64) (rs1_val : BitVec 64) :=
+  BitVec.and rs1_val (BitVec.not (BitVec.shiftLeft (BitVec.zeroExtend 64 1#1) (BitVec.extractLsb  5 0 rs2_val).toNat))
+
+
+def ZBB_EXTOP_pure64_RISCV_SEXTB (rs1_val : BitVec 64) :=
+  BitVec.signExtend 64 (BitVec.extractLsb 7 0 rs1_val)
+
+def ZBB_EXTOP_pure64_RISCV_SEXTH  (rs1_val : BitVec 64) :=
+  BitVec.signExtend 64 (BitVec.extractLsb 15 0 rs1_val)
+
+def ZBB_EXTOP_pure64_RISCV_ZEXTH  (rs1_val : BitVec 64) :=
+  BitVec.zeroExtend 64 (BitVec.extractLsb 15 0 rs1_val)
+
+def ZBS_RTYPE_pure64_RISCV_BEXT (rs2_val : BitVec 64) (rs1_val : BitVec 64)  :=
+  BitVec.setWidth 64
+    (match
+      BitVec.and rs1_val (BitVec.shiftLeft (BitVec.setWidth 64 1#1) (BitVec.extractLsb 5 0 rs2_val).toNat) !=
+        0#64 with
+    | true => 1#1
+    | false => 0#1)
+
+ def ZBS_RTYPE_pure64_BINV (rs2_val : BitVec 64) (rs1_val : BitVec 64) :=
+  BitVec.xor rs1_val  (BitVec.shiftLeft (BitVec.zeroExtend 64 1#1) (BitVec.extractLsb 5 0 rs2_val).toNat)
+
+def ZBS_RTYPE_pure64_RISCV_BSET (rs2_val : BitVec 64) (rs1_val : BitVec 64) :=
+  BitVec.or rs1_val (BitVec.shiftLeft (BitVec.zeroExtend 64 1#1) (BitVec.extractLsb 5 0 rs2_val).toNat)
+
+def ZBS_IOP_pure64_RISCV_BCLRI (shamt : BitVec 6) (rs1_val : BitVec 64) :=
+  BitVec.and rs1_val (BitVec.not (BitVec.shiftLeft (BitVec.setWidth 64 1#1) (shamt.toNat)))
+
+def ZBS_IOP_pure64_RISCV_BEXTI (shamt : BitVec 6) (rs1_val : BitVec 64) :=
+  BitVec.setWidth 64
+      (match (BitVec.and (rs1_val) (BitVec.shiftLeft (BitVec.setWidth 64 1#1) shamt.toNat)) != 0#64 with
+      | true => 1#1
+      | false => 0#1)
+
+def ZBS_IOP_pure64_RISCV_BINVI (shamt : BitVec 6) (rs1_val : BitVec 64) :=
+  BitVec.xor rs1_val  (BitVec.shiftLeft (BitVec.zeroExtend 64 1#1) shamt.toNat)
+
+def ZBS_IOP_pure64_RISCV_BSETI (shamt : BitVec 6) (rs1_val : BitVec 64) :=
+  BitVec.or rs1_val (BitVec.shiftLeft (BitVec.zeroExtend 64 1#1) shamt.toNat)
+
+def ZBB_RTYPEW_pure64_RISCV_RORW (rs2_val : BitVec 64) (rs1_val : BitVec 64) :=
+  BitVec.signExtend (64)
+      (BitVec.or (BitVec.ushiftRight (BitVec.setWidth 32 rs1_val) (rs2_val.toNat % 32))
+        (BitVec.shiftLeft (BitVec.setWidth 32 rs1_val)
+          ((2 ^ 5 - rs2_val.toNat % 32 +
+              32 % 2 ^ (5 + 1)) %
+            2 ^ 5)))
+
+def ZBB_RTYPEW_pure64_RISCV_ROLW (rs2_val : BitVec 64) (rs1_val : BitVec 64) :=
+BitVec.signExtend 64
+    (BitVec.or (BitVec.shiftLeft (BitVec.setWidth 32 rs1_val) (BitVec.extractLsb 4 0 rs2_val).toNat)
+      (BitVec.ushiftRight (BitVec.setWidth 32 rs1_val) (
+        ((BitVec.sub ((BitVec.extractLsb' 0 (5)
+            (BitVec.ofInt (6)
+              (32))))
+          (BitVec.extractLsb 4 0 rs2_val)))).toNat))
+
+ def ZBB_RTYPE_pure64_RISCV_ROL (rs2_val : BitVec 64) (rs1_val : BitVec 64) :=
+  BitVec.or (BitVec.shiftLeft  rs1_val (BitVec.extractLsb 5 0 rs2_val).toNat)
+    (BitVec.ushiftRight rs1_val  (BitVec.extractLsb' 0 6 (BitVec.ofInt (7) (64)) - BitVec.extractLsb 5 0 rs2_val).toNat)
+
+ def ZBB_RTYPE_pure64_RISCV_ROR (rs2_val : BitVec 64) (rs1_val : BitVec 64) :=
+      BitVec.or (BitVec.ushiftRight rs1_val (BitVec.extractLsb 5 0 rs2_val).toNat)
+    (BitVec.shiftLeft rs1_val ((BitVec.extractLsb' 0 6 (BitVec.ofInt (7) (64)) - BitVec.extractLsb 5 0 rs2_val)).toNat)
+/-
+|binv
+|bset
+|bclri
+|bexti
+|binvi
+|bseti
+|sext.b
+|sext.h
+|zext.h
+|rolw
+|rorw
+-/
+end RV64Semantics
