RiscvDialect/RISCV64/Syntax.lean
@@ -1,0 +1,597 @@
+import SSA.Core.MLIRSyntax.EDSL
+import RiscvDialect.RISCV64.Base
+
+open MLIR AST Ctxt
+open RISCV64
+
+namespace RISCVExpr
+
+def const {Γ : Ctxt _} (n : ℤ) : Expr RV64 Γ .pure .bv  :=
+  Expr.mk
+    (op := Op.const n)
+    (eff_le := by constructor)
+    (ty_eq := rfl)
+    (args := .nil)
+    (regArgs := HVector.nil)
+-- this is to easily write IR by hand
+-- alterantive would work :: Γ.Var .bv
+def add {Γ : Ctxt _} (e₁ e₂: Ctxt.Var Γ .bv) : Expr RV64 Γ .pure .bv  :=
+  Expr.mk
+    (op := Op.add)
+    (eff_le := by constructor)
+    (ty_eq := rfl)
+    (args := .cons e₁ <| .cons e₂ .nil)
+    (regArgs := HVector.nil)
+
+def sub {Γ : Ctxt _} (e₁ e₂: Ctxt.Var Γ .bv) : Expr RV64 Γ .pure .bv  :=
+  Expr.mk
+    (op := Op.sub)
+    (eff_le := by constructor)
+    (ty_eq := rfl)
+    (args := .cons e₁ <| .cons e₂ .nil) -- debug
+    (regArgs := HVector.nil)
+
+def and {Γ : Ctxt _} (e₁ e₂: Ctxt.Var Γ .bv) : Expr RV64 Γ .pure .bv  :=
+  Expr.mk
+    (op := Op.and)
+    (eff_le := by constructor)
+    (ty_eq := rfl)
+    (args := .cons e₁ <| .cons e₂ .nil)
+    (regArgs := HVector.nil)
+
+end RISCVExpr
+/-
+  |.sra, regs, _  => RV64.RTYPE_pure64_RISCV_SRA (regs.getN 0 (by simp [DialectSignature.sig, signature]))  (regs.getN 1 (by simp [DialectSignature.sig, signature]))
+  |.srai shamt, regs, _  => RV64.SHIFTIOP_pure64_RISCV_SRAI shamt  (regs.getN 0 (by simp [DialectSignature.sig, signature]))
+-/
+
+-- string representation of MLIR type into corresponding RISCV type
+def mkTy : MLIR.AST.MLIRType φ → MLIR.AST.ExceptM RV64 RV64.Ty
+  | MLIR.AST.MLIRType.undefined s => do
+    match s with
+    | "i64" => return .bv
+    | _ => throw .unsupportedType
+  | _ => throw .unsupportedType
+
+--#eval mkTy (MLIR.AST.MLIRType.undefined "BitVec_64")
+
+instance instTransformTy : MLIR.AST.TransformTy RV64 0 where
+  mkTy := mkTy
+
+#check Expr.mk
+#check mkTy
+
+def mkExpr (Γ : Ctxt _) (opStx : MLIR.AST.Op 0) :
+  MLIR.AST.ReaderM (RV64) (Σ eff ty, Expr (RV64) Γ eff ty) := do
+    match opStx.args with
+    | []  => do
+        let some att := opStx.attrs.getAttr "val"
+          | throw <| .unsupportedOp s!"no attirbute in const {repr opStx}"
+        match att with
+          | .int val ty =>
+            let opTy@(.bv) ← mkTy ty -- ty.mkTy
+            return ⟨.pure, opTy, ⟨
+              .const (val),
+              by
+              simp[DialectSignature.outTy, signature]
+             ,
+              by constructor,
+              .nil,
+              .nil
+            ⟩⟩
+          | _ => throw <| .unsupportedOp s!"unsupported operation {repr opStx}"
+    | v₁Stx::[] =>
+       let ⟨ty₁, v₁⟩ ← MLIR.AST.TypedSSAVal.mkVal Γ v₁Stx
+        match ty₁, opStx.name with
+        | .bv, "RV64.srai" => do
+          let some att := opStx.attrs.getAttr "shamt"
+             | throw <| .unsupportedOp s!"no attirbute in srai {repr opStx}"
+          match att with
+          | .int val ty => -- ides modell it as a list of 3 bools
+            let opTy@(.bv) ← mkTy ty -- ty.mkTy
+            return ⟨.pure, opTy, ⟨
+              .srai (BitVec.ofInt 6 val),
+              by
+              simp[DialectSignature.outTy, signature]
+             ,
+              by constructor,
+              .cons v₁ <| .nil,
+              .nil
+            ⟩⟩
+          | _ => throw <| .unsupportedOp s!"unsupported operation {repr opStx}"
+        | .bv, "RV64.bclri" => do
+          let some att := opStx.attrs.getAttr "imm"
+            | throw <| .unsupportedOp s!"no attirbute in bclri {repr opStx}"
+          match att with
+          | .int val ty => -- ides modell it as a list of 3 bools
+            let opTy@(.bv) ← mkTy ty -- ty.mkTy
+            return ⟨.pure, opTy, ⟨
+              .bclri (BitVec.ofInt 6 val),
+              by
+              simp[DialectSignature.outTy, signature]
+             ,
+              by constructor,
+              .cons v₁ <| .nil,
+              .nil
+            ⟩⟩
+          | _ => throw <| .unsupportedOp s!"unsupported operation {repr opStx}"
+        | .bv, "RV64.bexti" => do
+          let some att := opStx.attrs.getAttr "imm"
+            | throw <| .unsupportedOp s!"no attirbute in bexti {repr opStx}"
+          match att with
+          | .int val ty => -- ides modell it as a list of 3 bools
+            let opTy@(.bv) ← mkTy ty -- ty.mkTy
+            return ⟨.pure, opTy, ⟨
+              .bexti (BitVec.ofInt 6 val),
+              by
+              simp[DialectSignature.outTy, signature]
+             ,
+              by constructor,
+              .cons v₁ <| .nil,
+              .nil
+            ⟩⟩
+          | _ => throw <| .unsupportedOp s!"unsupported operation {repr opStx}"
+        | .bv, "RV64.bseti" => do
+          let some att := opStx.attrs.getAttr "imm"
+            | throw <| .unsupportedOp s!"no attirbute in bseti {repr opStx}"
+          match att with
+          | .int val ty => -- ides modell it as a list of 3 bools
+            let opTy@(.bv) ← mkTy ty -- ty.mkTy
+            return ⟨.pure, opTy, ⟨
+              .bseti (BitVec.ofInt 6 val),
+              by
+              simp[DialectSignature.outTy, signature]
+             ,
+              by constructor,
+              .cons v₁ <| .nil,
+              .nil
+            ⟩⟩
+          | _ => throw <| .unsupportedOp s!"unsupported operation {repr opStx}"
+        | .bv, "RV64.binvi" => do
+          let some att := opStx.attrs.getAttr "imm"
+            | throw <| .unsupportedOp s!"no attirbute in binvi {repr opStx}"
+          match att with
+          | .int val ty => -- ides modell it as a list of 3 bools
+            let opTy@(.bv) ← mkTy ty -- ty.mkTy
+            return ⟨.pure, opTy, ⟨
+              .binvi (BitVec.ofInt 6 val),
+              by
+              simp[DialectSignature.outTy, signature]
+             ,
+              by constructor,
+              .cons v₁ <| .nil,
+              .nil
+            ⟩⟩
+          | _ => throw <| .unsupportedOp s!"unsupported operation {repr opStx}"
+        | .bv, "RV64.addiw" => do
+          let some att := opStx.attrs.getAttr "imm"
+            | throw <| .unsupportedOp s!"no attirbute in addiw {repr opStx}"
+          match att with
+          | .int val ty =>
+            let opTy@(.bv) ← mkTy ty -- ty.mkTy
+            return ⟨.pure, opTy, ⟨
+              .addiw (BitVec.ofInt 12 val),
+              by
+              simp[DialectSignature.outTy, signature]
+             ,
+              by constructor,
+              .cons v₁ <| .nil,
+             -- .cons v₁ ::ₕ .nil,-- ask for what is this
+              .nil --
+            ⟩⟩
+          | _ => throw <| .unsupportedOp s!"unsupported operation {repr opStx}"
+        | .bv, "RV64.lui" => do
+          let some att := opStx.attrs.getAttr "imm"
+            | throw <| .unsupportedOp s!"no attirbute in lui {repr opStx}"
+          match att with
+          | .int val ty =>
+            let opTy@(.bv) ← mkTy ty -- ty.mkTy
+            return ⟨.pure, opTy, ⟨
+              .lui (BitVec.ofInt 20 val),
+              by
+              simp[DialectSignature.outTy, signature]
+             ,
+              by constructor,
+              .cons v₁ <| .nil,
+             -- .cons v₁ ::ₕ .nil,-- ask for what is this
+              .nil --
+            ⟩⟩
+          | _ => throw <| .unsupportedOp s!"unsupported operation {repr opStx}"
+        | .bv, "RV64.auipc" => do
+          let some att := opStx.attrs.getAttr "imm"
+            | throw <| .unsupportedOp s!"no attirbute in auipc {repr opStx}"
+          match att with
+          | .int val ty =>
+            let opTy@(.bv) ← mkTy ty -- ty.mkTy
+            return ⟨.pure, opTy, ⟨
+              .auipc (BitVec.ofInt 20 val),
+              by
+              simp[DialectSignature.outTy, signature]
+             ,
+              by constructor,
+              .cons v₁ <| .nil,
+              .nil
+            ⟩⟩
+          | _ => throw <| .unsupportedOp s!"unsupported operation {repr opStx}"
+        | .bv, "RV64.slliw" => do
+          let some att := opStx.attrs.getAttr "shamt"
+            | throw <| .unsupportedOp s!"no attirbute in slliw {repr opStx}"
+          match att with
+          | .int val ty => -- ides modell it as a list of 3 bools
+            let opTy@(.bv) ← mkTy ty -- ty.mkTy
+            return ⟨.pure, opTy, ⟨
+              .slliw (BitVec.ofInt 5 val),
+              by
+              simp[DialectSignature.outTy, signature]
+             ,
+              by constructor,
+              .cons v₁ <| .nil,
+              .nil
+            ⟩⟩
+          | _ => throw <| .unsupportedOp s!"unsupported operation {repr opStx}"
+        | .bv, "RV64.srliw" => do
+          let some att := opStx.attrs.getAttr "shamt"
+            | throw <| .unsupportedOp s!"no attirbute in slliw {repr opStx}"
+          match att with
+          | .int val ty =>
+            let opTy@(.bv) ← mkTy ty -- ty.mkTy
+            return ⟨.pure, opTy, ⟨
+              .srliw (BitVec.ofInt 5 val),
+              by
+              simp[DialectSignature.outTy, signature]
+             ,
+              by constructor,
+              .cons v₁ <| .nil,
+              .nil
+            ⟩⟩
+          | _ => throw <| .unsupportedOp s!"unsupported operation {repr opStx}"
+        | .bv, "RV64.sraiw" => do
+          let some att := opStx.attrs.getAttr "shamt"
+            | throw <| .unsupportedOp s!"no attirbute in sraiw {repr opStx}"
+          match att with
+          | .int val ty =>
+            let opTy@(.bv) ← mkTy ty -- ty.mkTy
+            return ⟨.pure, opTy, ⟨
+              .sraiw (BitVec.ofInt 5 val),
+              by
+              simp[DialectSignature.outTy, signature]
+             ,
+              by constructor,
+              .cons v₁ <| .nil,
+              .nil
+            ⟩⟩
+          | _ => throw <| .unsupportedOp s!"unsupported operation {repr opStx}"
+        | .bv, "RV64.slli" => do
+          let some att := opStx.attrs.getAttr "shamt"
+            | throw <| .unsupportedOp s!"no attirbute in slli{repr opStx}"
+          match att with
+          | .int val ty =>
+            let opTy@(.bv) ← mkTy ty -- ty.mkTy
+            return ⟨.pure, opTy, ⟨
+              .slli (BitVec.ofInt 6 val),
+              by
+              simp[DialectSignature.outTy, signature]
+             ,
+              by constructor,
+              .cons v₁ <| .nil,
+              .nil
+            ⟩⟩
+          | _ => throw <| .unsupportedOp s!"unsupported operation {repr opStx}"
+        | .bv, "RV64.srli" => do
+          let some att := opStx.attrs.getAttr "shamt"
+            | throw <| .unsupportedOp s!"no attirbute in srli {repr opStx}"
+          match att with
+          | .int val ty =>
+            let opTy@(.bv) ← mkTy ty -- ty.mkTy
+            return ⟨.pure, opTy, ⟨
+              .srli (BitVec.ofInt 6 val),
+              by
+              simp[DialectSignature.outTy, signature]
+             ,
+              by constructor,
+              .cons v₁ <| .nil,
+              .nil
+            ⟩⟩
+          | _ => throw <| .unsupportedOp s!"unsupported operation {repr opStx}"
+        | .bv, "RV64.addi" => do
+          let some att := opStx.attrs.getAttr "imm"
+            | throw <| .unsupportedOp s!"no attirbute in addi {repr opStx}"
+          match att with
+          | .int val ty =>
+            let opTy@(.bv) ← mkTy ty -- ty.mkTy
+            return ⟨.pure, opTy, ⟨
+              .addi (BitVec.ofInt 12 val),
+              by
+              simp[DialectSignature.outTy, signature]
+             ,
+              by constructor,
+              .cons v₁ <| .nil,
+             -- .cons v₁ ::ₕ .nil,-- ask for what is this
+              .nil --
+            ⟩⟩
+          | _ => throw <| .unsupportedOp s!"unsupported operation {repr opStx}"
+        | .bv, "RV64.slti" => do
+          let some att := opStx.attrs.getAttr "imm"
+            | throw <| .unsupportedOp s!"no attirbute in slti {repr opStx}"
+          match att with
+          | .int val ty =>
+            let opTy@(.bv) ← mkTy ty -- ty.mkTy
+            return ⟨.pure, opTy, ⟨
+              .slti (BitVec.ofInt 12 val),
+              by
+              simp[DialectSignature.outTy, signature]
+             ,
+              by constructor,
+              .cons v₁ <| .nil,
+             -- .cons v₁ ::ₕ .nil,-- ask for what is this
+              .nil --
+            ⟩⟩
+          | _ => throw <| .unsupportedOp s!"unsupported operation {repr opStx}"
+        | .bv, "RV64.sltiu" => do
+          let some att := opStx.attrs.getAttr "imm"
+            | throw <| .unsupportedOp s!"no attirbute in sltiu {repr opStx}"
+          match att with
+          | .int val ty =>
+            let opTy@(.bv) ← mkTy ty -- ty.mkTy
+            return ⟨.pure, opTy, ⟨
+              .sltiu (BitVec.ofInt 12 val),
+              by
+              simp[DialectSignature.outTy, signature]
+             ,
+              by constructor,
+              .cons v₁ <| .nil,
+             -- .cons v₁ ::ₕ .nil,-- ask for what is this
+              .nil --
+            ⟩⟩
+          | _ => throw <| .unsupportedOp s!"unsupported operation {repr opStx}"
+        | .bv, "RV64.andi" => do
+          let some att := opStx.attrs.getAttr "imm"
+            | throw <| .unsupportedOp s!"no attirbute in andi {repr opStx}"
+          match att with
+          | .int val ty =>
+            let opTy@(.bv) ← mkTy ty -- ty.mkTy
+            return ⟨.pure, opTy, ⟨
+              .andi (BitVec.ofInt 12 val),
+              by
+              simp[DialectSignature.outTy, signature]
+             ,
+              by constructor,
+              .cons v₁ <| .nil,
+             -- .cons v₁ ::ₕ .nil,-- ask for what is this
+              .nil --
+            ⟩⟩
+          | _ => throw <| .unsupportedOp s!"unsupported operation {repr opStx}"
+        | .bv, "RV64.ori" => do
+          let some att := opStx.attrs.getAttr "imm"
+            | throw <| .unsupportedOp s!"no attirbute in ori {repr opStx}"
+          match att with
+          | .int val ty =>
+            let opTy@(.bv) ← mkTy ty -- ty.mkTy
+            return ⟨.pure, opTy, ⟨
+              .ori (BitVec.ofInt 12 val),
+              by
+              simp[DialectSignature.outTy, signature]
+             ,
+              by constructor,
+              .cons v₁ <| .nil,
+             -- .cons v₁ ::ₕ .nil,-- ask for what is this
+              .nil --
+            ⟩⟩
+          | _ => throw <| .unsupportedOp s!"unsupported operation {repr opStx}"
+        | .bv, "RV64.xori" => do
+          let some att := opStx.attrs.getAttr "imm"
+            | throw <| .unsupportedOp s!"no attirbute in ori {repr opStx}"
+          match att with
+          | .int val ty =>
+            let opTy@(.bv) ← mkTy ty -- ty.mkTy
+            return ⟨.pure, opTy, ⟨
+              .xori (BitVec.ofInt 12 val),
+              by
+              simp[DialectSignature.outTy, signature]
+             ,
+              by constructor,
+              .cons v₁ <| .nil,
+             -- .cons v₁ ::ₕ .nil,-- ask for what is this
+              .nil --
+            ⟩⟩
+          | _ => throw <| .unsupportedOp s!"unsupported operation {repr opStx}"
+        | .bv, "RV64.sext.b" =>
+            return ⟨ .pure, .bv ,⟨ .sext.b, by rfl, by constructor,
+               .cons v₁ <| .nil,
+                .nil⟩⟩
+        | .bv, "RV64.sext.h" =>
+            return ⟨ .pure, .bv ,⟨ .sext.h, by rfl, by constructor,
+               .cons v₁ <| .nil,
+                .nil⟩⟩
+        | .bv, "RV64.zext.h" =>
+            return ⟨ .pure, .bv ,⟨ .zext.h, by rfl, by constructor,
+               .cons v₁ <| .nil,
+                .nil⟩⟩
+        |_ , _ => throw <| .unsupportedOp s!"unsupported operation {repr opStx}"
+    | v₁Stx::v₂Stx:: [] =>
+        let ⟨ty₁, v₁⟩ ← MLIR.AST.TypedSSAVal.mkVal Γ v₁Stx
+        let ⟨ty₂, v₂⟩ ← MLIR.AST.TypedSSAVal.mkVal Γ v₂Stx
+        match ty₁, ty₂, opStx.name with
+        | .bv, .bv, "RV64.rem" =>
+          return ⟨.pure, .bv ,⟨ .rem, by rfl ,by constructor,
+             .cons v₁ <| .cons v₂ <| .nil,
+              .nil ⟩⟩
+        | .bv, .bv, "RV64.ror" =>
+          return ⟨.pure, .bv ,⟨ .ror, by rfl ,by constructor,
+             .cons v₁ <| .cons v₂ <| .nil,
+              .nil ⟩⟩
+        | .bv, .bv, "RV64.rol" =>
+          return ⟨.pure, .bv ,⟨ .rol, by rfl ,by constructor,
+             .cons v₁ <| .cons v₂ <| .nil,
+              .nil ⟩⟩
+        | .bv, .bv, "RV64.remu" =>
+          return ⟨.pure, .bv ,⟨ .remu, by rfl ,by constructor,
+             .cons v₁ <| .cons v₂ <| .nil,
+              .nil ⟩⟩
+        | .bv, .bv, "RV64.sra" =>
+          return ⟨.pure, .bv ,⟨ .sra, by rfl ,by constructor,
+             .cons v₁ <| .cons v₂ <| .nil,
+              .nil ⟩⟩
+        | .bv, .bv, "RV64.addw" =>
+          return ⟨.pure, .bv ,⟨ .addw, by rfl ,by constructor,
+             .cons v₁ <| .cons v₂ <| .nil,
+              .nil ⟩⟩
+        | .bv , .bv , "RV64.subw" =>
+              return ⟨ .pure, .bv ,⟨ .subw, by rfl, by constructor,
+               .cons v₁ <| .cons v₂ <| .nil,
+                .nil⟩⟩
+        | .bv , .bv , "RV64.sllw" =>
+              return ⟨ .pure, .bv ,⟨ .sllw, by rfl, by constructor,
+               .cons v₁ <| .cons v₂ <| .nil,
+                .nil⟩⟩
+        | .bv , .bv , "RV64.srlw" =>
+              return ⟨ .pure, .bv ,⟨ .srlw, by rfl, by constructor,
+               .cons v₁ <| .cons v₂ <| .nil,
+                .nil⟩⟩
+        | .bv , .bv , "RV64.sraw" =>
+              return ⟨ .pure, .bv ,⟨ .sraw, by rfl, by constructor,
+               .cons v₁ <| .cons v₂ <| .nil,
+                .nil⟩⟩
+        | .bv , .bv , "RV64.add" =>
+              return ⟨ .pure, .bv ,⟨ .add, by rfl, by constructor,
+               .cons v₁ <| .cons v₂ <| .nil,
+                .nil⟩⟩
+        | .bv , .bv , "RV64.or" =>
+              return ⟨ .pure, .bv ,⟨ .or, by rfl, by constructor,
+               .cons v₁ <| .cons v₂ <| .nil,
+                .nil⟩⟩
+        | .bv , .bv , "RV64.xor" =>
+              return ⟨ .pure, .bv ,⟨ .xor, by rfl, by constructor,
+               .cons v₁ <| .cons v₂ <| .nil,
+                .nil⟩⟩
+        | .bv , .bv , "RV64.sll" =>
+              return ⟨ .pure, .bv ,⟨ .sll, by rfl, by constructor,
+               .cons v₁ <| .cons v₂ <| .nil,
+                .nil⟩⟩
+        | .bv , .bv , "RV64.srl" =>
+              return ⟨ .pure, .bv ,⟨ .srl, by rfl, by constructor,
+               .cons v₁ <| .cons v₂ <| .nil,
+                .nil⟩⟩
+        | .bv , .bv , "RV64.sub" =>
+              return ⟨ .pure, .bv ,⟨ .sub, by rfl, by constructor,
+               .cons v₁ <| .cons v₂ <| .nil,
+                .nil⟩⟩
+        | .bv , .bv , "RV64.slt" =>
+              return ⟨ .pure, .bv ,⟨ .slt, by rfl, by constructor,
+               .cons v₁ <| .cons v₂ <| .nil,
+                .nil⟩⟩
+        | .bv , .bv , "RV64.sltu" =>
+              return ⟨ .pure, .bv ,⟨ .sltu, by rfl, by constructor,
+               .cons v₁ <| .cons v₂ <| .nil,
+                .nil⟩⟩
+        | .bv , .bv , "RV64.and" =>
+              return ⟨ .pure, .bv ,⟨ .and, by rfl, by constructor,
+               .cons v₁ <| .cons v₂ <| .nil,
+                .nil⟩⟩
+        | .bv , .bv , "RV64.czero.eqz" =>
+              return ⟨ .pure, .bv ,⟨ .czero.eqz, by rfl, by constructor,
+               .cons v₁ <| .cons v₂ <| .nil,
+                .nil⟩⟩
+        | .bv , .bv , "RV64.czero.nez" =>
+              return ⟨ .pure, .bv ,⟨ .czero.nez, by rfl, by constructor,
+               .cons v₁ <| .cons v₂ <| .nil,
+                .nil⟩⟩
+        | .bv , .bv , "RV64.bclr" =>
+              return ⟨ .pure, .bv ,⟨ .bclr, by rfl, by constructor,
+               .cons v₁ <| .cons v₂ <| .nil,
+                .nil⟩⟩
+        | .bv , .bv , "RV64.bext" =>
+              return ⟨ .pure, .bv ,⟨ .bext, by rfl, by constructor,
+               .cons v₁ <| .cons v₂ <| .nil,
+                .nil⟩⟩
+        | .bv , .bv , "RV64.binv" =>
+              return ⟨ .pure, .bv ,⟨ .binv, by rfl, by constructor,
+               .cons v₁ <| .cons v₂ <| .nil,
+                .nil⟩⟩
+        | .bv , .bv , "RV64.bset" =>
+              return ⟨ .pure, .bv ,⟨ .bset, by rfl, by constructor,
+               .cons v₁ <| .cons v₂ <| .nil,
+                .nil⟩⟩
+        | .bv , .bv , "RV64.rolw" =>
+              return ⟨ .pure, .bv ,⟨ .rolw, by rfl, by constructor,
+               .cons v₁ <| .cons v₂ <| .nil,
+                .nil⟩⟩
+        | .bv , .bv , "RV64.rorw" =>
+              return ⟨ .pure, .bv ,⟨ .rorw, by rfl, by constructor,
+               .cons v₁ <| .cons v₂ <| .nil,
+                .nil⟩⟩
+        | .bv , .bv , "RV64.mul" =>
+            return ⟨ .pure, .bv ,⟨ .mul, by rfl, by constructor,
+               .cons v₁ <| .cons v₂ <| .nil,
+                .nil⟩⟩
+        | .bv , .bv , "RV64.mulu" =>
+            return ⟨ .pure, .bv ,⟨ .mulu, by rfl, by constructor,
+               .cons v₁ <| .cons v₂ <| .nil,
+                .nil⟩⟩
+        | .bv , .bv , "RV64.mulh" =>
+            return ⟨ .pure, .bv ,⟨ .mulh, by rfl, by constructor,
+               .cons v₁ <| .cons v₂ <| .nil,
+                .nil⟩⟩
+        | .bv , .bv , "RV64.mulhu" =>
+            return ⟨ .pure, .bv ,⟨ .mulhu, by rfl, by constructor,
+               .cons v₁ <| .cons v₂ <| .nil,
+                .nil⟩⟩
+        | .bv , .bv , "RV64.mulhsu" =>
+            return ⟨ .pure, .bv ,⟨ .mulhsu, by rfl, by constructor,
+               .cons v₁ <| .cons v₂ <| .nil,
+                .nil⟩⟩
+
+        | .bv , .bv , "RV64.mulw" => do -- (s : Bool)
+          return ⟨ .pure, .bv ,⟨ .mulw, by rfl, by constructor,
+               .cons v₁ <| .cons v₂ <| .nil,
+                .nil⟩⟩
+        | .bv, .bv, "RV64.divw" =>
+          return ⟨ .pure, .bv ,⟨ .divw, by rfl, by constructor,
+               .cons v₁ <| .cons v₂ <| .nil,
+                .nil⟩⟩
+        | .bv, .bv, "RV64.divwu" =>
+            return ⟨ .pure, .bv ,⟨ .divwu, by rfl, by constructor,
+               .cons v₁ <| .cons v₂ <| .nil,
+                .nil⟩⟩
+        | .bv, .bv, "RV64.div" =>
+            return ⟨ .pure, .bv ,⟨ .div, by rfl, by constructor,
+               .cons v₁ <| .cons v₂ <| .nil,
+                .nil⟩⟩
+        | .bv, .bv, "RV64.divu" =>
+            return ⟨ .pure, .bv ,⟨ .divu, by rfl, by constructor,
+               .cons v₁ <| .cons v₂ <| .nil,
+                .nil⟩⟩
+        | .bv, .bv, "RV64.remw" =>
+            return ⟨ .pure, .bv ,⟨ .remw, by rfl, by constructor,
+               .cons v₁ <| .cons v₂ <| .nil,
+                .nil⟩⟩
+        | .bv, .bv, "RV64.remwu" =>
+            return ⟨ .pure, .bv ,⟨ .remw, by rfl, by constructor,
+               .cons v₁ <| .cons v₂ <| .nil,
+                .nil⟩⟩
+
+
+        | _, _ , _ => throw <| .unsupportedOp s!"type mismatch  for 2 reg operation  {repr opStx}"
+    | _ => throw <| .unsupportedOp s!"wrong number of arguemnts, more than 2 arguemnts  {repr opStx}"
+
+instance : MLIR.AST.TransformExpr (RV64) 0 where
+  mkExpr := mkExpr
+
+def mkReturn (Γ : Ctxt _) (opStx : MLIR.AST.Op 0) : MLIR.AST.ReaderM (RV64)
+    (Σ eff ty, Com RV64 Γ eff ty) :=
+  if opStx.name == "return"
+  then match opStx.args with
+  | vStx::[] => do
+    let ⟨ty, v⟩ ← MLIR.AST.TypedSSAVal.mkVal Γ vStx
+    return ⟨.pure, ty, Com.ret v⟩
+  | _ => throw <| .generic s!"Ill-formed return statement (wrong arity, expected 1, got {opStx.args.length})"
+  else throw <| .generic s!"Tried to build return out of non-return statement {opStx.name}"
+
+
+instance : MLIR.AST.TransformReturn (RV64) 0 where
+  mkReturn := mkReturn
+
+
+open Qq MLIR AST Lean Elab Term Meta in
+elab "[RV64_com| " reg:mlir_region "]" : term => do
+  SSA.elabIntoCom reg q(RV64)
