thesis_examples/background/examples-bitvec-bvdecide.lean
@@ -1,0 +1,4 @@
+def exampleFin : Fin 64  := ⟨ 19 , by simp [Nat.reduceLT]⟩ -- Fin,
+def bv32_ex1 : BitVec 32 :=  ⟨42, by simp [Nat.reducePow, Nat.reduceLT]⟩
+def bv32_ex2 : BitVec 32 :=  42#32
+def bv32_ex3 : BitVec 32 :=  BitVec.ofNat 32 43
